Final version

ex2bonus.v
@@ -5,15 +5,450 @@ Import ListNotations.
 Require Import Arith.EqNat.
 Require Import Arith.Le.
 
+(** Defining some functions on natural integers **)
+
+Definition change_val (A : Type) (f : nat -> A) (x : nat) (a : A) : nat -> A :=
+  fun (y : nat) => if Nat.eqb x y then a else f y.
+
+Lemma change_val_refl (A : Type) (f : nat -> A) (x : nat) (a : A) :
+  change_val f x a x = a.
+Proof.
+  unfold change_val.
+  rewrite Nat.eqb_refl with (x := x).
+  reflexivity.
+Qed.
+
+Fixpoint remove_nat (A : Type) (x : nat) (f : nat -> A) (offset : nat) (default : A) (y : nat) : A :=
+  match x with
+  | 0 => match y with
+         | 0 => default
+         | S y => f (offset + y)
+         end
+  | S x => match y with
+         | 0 => f offset
+         | S y => remove_nat x f (S offset) default y
+         end
+  end.
+
+Lemma remove_nat_gt (A : Type) (x : nat) (f : nat -> A) (default : A) (y : nat) :
+  x <= y -> remove_nat x f 0 default (S y) = f y.
+Proof.
+  remember (f y) as fy.
+  rewrite <- Nat.add_0_l with (n := y) in Heqfy.
+  rewrite Heqfy.
+  clear fy Heqfy.
+  generalize 0 as offset.
+  revert y.
+  induction x; intro y.
+  - destruct y; reflexivity.
+  - destruct y; intros offset Hle.
+    + contradiction (Nat.nle_succ_0 x Hle).
+    + rewrite <- Nat.add_succ_comm with (n := offset) (m := y).
+      apply IHx.
+      apply le_S_n.
+      apply Hle.
+Qed.
+
+Lemma remove_nat_lt (A : Type) (x : nat) (f : nat -> A) (default : A) (y : nat) :
+  y < x -> remove_nat x f 0 default y = f y.
+Proof.
+  remember (f y) as fy.
+  rewrite <- Nat.add_0_l with (n := y) in Heqfy.
+  rewrite Heqfy.
+  clear fy Heqfy.
+  generalize 0 as offset.
+  revert y.
+  induction x; intro y.
+  - intros offset Hlt.
+    contradiction (Nat.nle_succ_0 y Hlt).
+  - destruct y; intros offset Hle.
+    + rewrite Nat.add_0_r with (n := offset).
+      reflexivity.
+    + rewrite <- Nat.add_succ_comm with (n := offset) (m := y).
+      apply IHx.
+      apply le_S_n.
+      apply Hle.
+Qed.
+
+Lemma remove_nat_eq (A : Type) (x : nat) (f : nat -> A) (default : A) :
+  remove_nat x f 0 default x = default.
+Proof.
+  generalize 0 as offset.
+  induction x; intro offset.
+  - reflexivity.
+  - apply IHx.
+Qed.
+
+Definition exchange_nat (x y z : nat) : nat :=
+  if Nat.eqb z x then y else if Nat.eqb z y then x else z.
+
+Lemma exchange_nat_l (x y : nat) :
+  exchange_nat x y x = y.
+Proof.
+  unfold exchange_nat.
+  rewrite (Nat.eqb_refl x).
+  reflexivity.
+Qed.
+
+Lemma exchange_nat_r (x y : nat) :
+  exchange_nat x y y = x.
+Proof.
+  unfold exchange_nat.
+  destruct (Bool.bool_dec (Nat.eqb y x) true) as [Eq | Neq].
+  - rewrite Eq.
+    apply Nat.eqb_eq.
+    assumption.
+  - apply Bool.not_true_iff_false in Neq.
+    rewrite Neq.
+    rewrite (Nat.eqb_refl y).
+    reflexivity.
+Qed.
+
+Lemma exchange_nat_inv (x y z : nat) :
+  exchange_nat x y (exchange_nat x y z) = z.
+Proof.
+  unfold exchange_nat.
+  destruct (Bool.bool_dec (Nat.eqb z x) true) as [Eq | Neq].
+  + rewrite Eq.
+    destruct (Bool.bool_dec (Nat.eqb y x) true) as [Eq1 | Neq1].
+    * rewrite Eq1.
+      apply eq_trans with (y := x).
+      apply Nat.eqb_eq.
+      assumption.
+      apply eq_sym.
+      apply Nat.eqb_eq.
+      assumption.
+    * apply Bool.not_true_iff_false in Neq1.
+      rewrite Neq1.
+      rewrite (Nat.eqb_refl y).
+      apply eq_sym.
+      apply Nat.eqb_eq.
+      assumption.
+  + apply Bool.not_true_iff_false in Neq.
+    rewrite Neq.
+    destruct (Bool.bool_dec (Nat.eqb z y) true) as [Eq1 | Neq1].
+    * rewrite Eq1.
+      rewrite (Nat.eqb_refl x).
+      apply eq_sym.
+      apply Nat.eqb_eq.
+      assumption.
+    * apply Bool.not_true_iff_false in Neq1.
+      rewrite Neq1.
+      rewrite Neq.
+      rewrite Neq1.
+      reflexivity.
+Qed.
+
+(** Encoding definable subsets of A as elements of type A -> Prop **)
+
+Inductive finite_set (A : Type) (l : list A) : A -> Prop :=
+  | Finite_set : forall (a : A), In a l -> finite_set l a.
+
+Inductive fun_image (A : Type) (f : A -> A) (P : A -> Prop) : A ->  Prop :=
+  | Fun_image : forall (a : A), P a -> fun_image f P (f a).
+
+
+(** Implementation of vect A n et fin n **)
+
+Inductive fin : nat -> Set :=
+  | Zero : forall (n : nat), fin (S n)
+  | Succ : forall (n : nat), fin n -> fin (S n).
+
+Inductive vect (A : Type) : nat -> Type :=
+  | Vnil : vect A 0
+  | Vcons : forall (n : nat), A -> vect A n -> vect A (S n).
+
+Fixpoint nat_to_fin (n m : nat) : m < n ->  fin n :=
+  match n with
+  | 0 => fun p => except ((Nat.nle_succ_0 m) p)
+  | S n => match m with
+           | 0 => fun p => Zero n
+           | S m => fun p => Succ (nat_to_fin (le_S_n (S m) n p))
+           end
+  end.
+
+Fixpoint fin_incl (n m : nat) : m <= n -> fin m -> fin n :=
+  match n with
+  | 0 => match m with
+         | 0 => fun _ t => t
+         | S m => fun p _ => except (Nat.nle_succ_0 m p)
+         end
+  | S n => match m with
+           | 0 => fun _ (t : fin 0) => match t in fin m return (match m with 0 => fin (S n) | S _ => unit end) with
+                             | Zero _ => tt
+                             | Succ _ => tt
+                             end
+           | S m => fun p t => let t := match t in fin (S m) return option (fin m) with
+                               | Zero _ => None
+                               | Succ t => Some t
+                               end in match t with
+                               | None => Zero n
+                               | Some t => Succ (fin_incl (le_S_n m n p) t)
+                               end
+           end
+  end.
+
+
+Fixpoint vect_proj (A : Type) (n m : nat) : m <= n -> vect A n -> vect A m :=
+  match n with
+  | 0 => match m with
+         | 0 => fun _ v => v
+         | S m => fun p _ => match (fin_incl p (Zero m)) in fin n0 return (match n0 with 0 => vect A (S m) | S _ => unit end) with
+                             | Zero _ => tt
+                             | Succ _ => tt
+                             end
+         end
+  | S n => match m with
+           | 0 => fun _ _ => Vnil A
+           | S m => fun p v => let (x,v) := (match v in vect _ (S n) return A * vect A n with
+                               | Vcons x v => (x,v)
+                               end) in Vcons x (vect_proj (le_S_n m n p) v)
+           end
+  end.
+
+Fixpoint Vnth (A : Type) (n : nat) (t : fin n) : vect A n -> A :=
+  match t with
+  | Zero n => fun v => match v with Vcons x _ => x end
+  | Succ t => fun v => Vnth t (match v with Vcons _ v => v end)
+  end.
+
+
+Lemma vect_proj_vnth (A : Type) (n m : nat) (p : m <= n) (t : fin m) (v : vect A n) :
+  Vnth t (vect_proj p v) = Vnth (fin_incl p t) v.
+Proof.
+  revert m t p.
+  induction v; intros m t.
+  - destruct t; intro p; contradiction (Nat.nle_succ_0 n p).
+  - destruct t; intro p.
+    + reflexivity.
+    + apply IHv.
+Qed.
+
+Fixpoint make_vect (A : Type) (n : nat) (x : A) : vect A n :=
+  match n with
+  | 0 => Vnil A
+  | S n => Vcons x (make_vect n x)
+  end.
+
+Fixpoint vect_app (A : Type) (n m : nat) (a0 : A) : m <= n -> vect A m -> vect A n :=
+  match n with
+  | 0 => match m with
+         | 0 => fun _ _ => Vnil A
+         | S m => fun (p : m < 0) _ => match fin_incl p (Zero m) in fin n0 return (match n0 with 0 => vect A 0 | S _ => unit end) with
+                                          | Zero _ => tt
+                                          | Succ _ => tt
+                                          end
+         end
+  | S n => match m with
+           | 0 => fun _ _ => make_vect (S n) a0
+           | S m => fun (p : S m <= S n) (v : vect A (S m)) => let (x,v') := match v in vect _ (S m) return A * vect A m with
+                                                                             | Vcons x v => (x,v)
+                                                                             end in Vcons x (vect_app a0 (le_S_n m n p) v')
+           end
+  end.
+
+Lemma vect_proj_app_inv (A : Type) (n m : nat) (a0 : A) (p : m <= n) (v : vect A m) :
+  vect_proj p (vect_app a0 p v) = v.
+Proof.
+  revert m p v.
+  induction n; intros m p v.
+  - induction v.
+    + reflexivity.
+    + contradiction (Nat.nle_succ_0 n p).
+  - induction v.
+    + reflexivity.
+    + simpl.
+      apply f_equal2 with (f := @Vcons A n0).
+      * reflexivity.
+      * apply IHn.
+Qed.
+
+Fixpoint insert (A : Type) (n m : nat) (a0 : A) : m <= n -> vect A n -> vect A (S n) :=
+  match m with
+  | 0 => fun _ => Vcons a0
+  | S m => match n with
+           | 0 => fun p _ => match fin_incl p (Zero m) in fin n0 return (match n0 with 0 => vect A 1 | S _ => unit end) with
+                             | Zero _ => tt
+                             | Succ _ => tt
+                             end
+           | S n => fun p v => let (x,v') := match v in vect _ (S n) return A * vect A n with
+                                           | Vcons x v => (x,v)
+                                           end in Vcons x (insert a0 (le_S_n m n p) v')
+           end
+  end.
+
+Lemma nat_to_fin_proof_irrelevance (n m : nat) (p q : m < n) :
+  nat_to_fin p = nat_to_fin q.
+Proof.
+  revert m p q.
+  induction n; intro m.
+  - intro p.
+    contradiction (Nat.nle_succ_0 m p).
+  - induction m; intros p q.
+    + reflexivity.
+    + simpl nat_to_fin.
+      apply f_equal.
+      apply IHn.
+Qed.
+
+Lemma insert_proof_irrelevance (A : Type) (n m : nat) (a0 : A) (p q : m <= n) :
+  insert a0 p = insert a0 q.
+Proof.
+  revert m p q.
+  induction n.
+  - destruct m; intros p q.
+    + reflexivity.
+    + contradiction (Nat.nle_succ_0 m p).
+  - destruct m; intros p q.
+    + reflexivity.
+    + simpl.
+      rewrite IHn with (p := le_S_n m n p) (q := le_S_n m n q).
+      reflexivity.
+Qed.
+
+Lemma insert_vnth_lt (A : Type) (n m o : nat) (a0 : A) (p : m <= n) (q : o < m) (v : vect A n) :
+  Vnth (nat_to_fin (le_S (S o) n (Nat.le_trans (S o) m n q p))) (insert a0 p v) = Vnth (nat_to_fin (Nat.le_trans (S o) m n q p)) v.
+Proof.
+  revert m p o q.
+  induction v; intro m.
+  - intros p o q.
+    contradiction (Nat.nle_succ_0 o (Nat.le_trans (S o) m 0 q p)).
+  - destruct m; intros p o q.
+    + contradiction (Nat.nle_succ_0 o q).
+    + destruct o.
+      * reflexivity.
+      * simpl insert.
+        simpl nat_to_fin.
+        simpl Vnth.
+        change (match o as m1 return (m1 < S n -> fin (S n)) with
+      | 0 => fun _ : 0 < S n => Zero n
+      | S m0 => fun p0 : S m0 < S n => Succ (nat_to_fin (n:=n) (m:=m0) (le_S_n (S m0) n p0))
+      end (le_S_n (S o) (S n) (le_S (S (S o)) (S n) (Nat.le_trans (S (S o)) (S m) (S n) q p)))) with (nat_to_fin (le_S_n (S o) (S n) (le_S (S (S o)) (S n) (Nat.le_trans (S (S o)) (S m) (S n) q p)))).
+        rewrite nat_to_fin_proof_irrelevance with (p := le_S_n (S o) (S n) (le_S (S (S o)) (S n) (Nat.le_trans (S (S o)) (S m) (S n) q p))) (q := le_S (S o) n (Nat.le_trans (S o) m n (le_S_n (S o) m q) (le_S_n m n p))).
+        rewrite nat_to_fin_proof_irrelevance with (p := le_S_n (S o) n (Nat.le_trans (S (S o)) (S m) (S n) q p)) (q := Nat.le_trans (S o) m n (le_S_n (S o) m q) (le_S_n m n p)).
+        apply IHv.
+Qed.
+
+Lemma insert_vnth_gt (A : Type) (n m o : nat) (a0 : A) (p : m <= o) (q : o < n) (v : vect A n) :
+  Vnth (nat_to_fin (le_n_S (S o) n q)) (insert a0 (Nat.le_trans m (S o) n (le_S m o p) q) v) = Vnth (nat_to_fin q) v.
+Proof.
+  revert o q m p.
+  induction v; intro o.
+  - intro q.
+    contradiction (Nat.nle_succ_0 o q).
+  - destruct o; intros q m.
+    + destruct m; intro p.
+      * reflexivity.
+      * contradiction (Nat.nle_succ_0 m p).
+    + destruct m; intro p.
+      * simpl.
+        apply f_equal with (f := fun t => Vnth t v).
+        apply nat_to_fin_proof_irrelevance.
+      * simpl insert.
+        change (nat_to_fin q) with (Succ (nat_to_fin (le_S_n (S o) n q))).
+        simpl Vnth.
+        apply eq_trans with (y := Vnth (nat_to_fin (le_S_n (S (S o)) (S n) (le_n_S (S (S o)) (S n) q))) (insert a0 (le_S_n m n (Nat.le_trans (S m) (S (S o)) (S n) (le_S (S m) (S o) p) q)) v)).
+          reflexivity.
+          rewrite nat_to_fin_proof_irrelevance with (p := le_S_n (S (S o)) (S n) (le_n_S (S (S o)) (S n) q)) (q := le_n_S (S o) n (le_S_n (S o) n q)).
+          rewrite insert_proof_irrelevance with (p := le_S_n m n (Nat.le_trans (S m) (S (S o)) (S n) (le_S (S m) (S o) p) q)) (q := Nat.le_trans m (S o) n (le_S m o (le_S_n m o p)) (le_S_n (S o) n q)).
+          apply IHv.
+Qed.
+
+Lemma insert_vnth_eq (A : Type) (n m : nat) (a0 : A) (p : m <= n) (v : vect A n) :
+  Vnth (nat_to_fin (le_n_S m n p)) (insert a0 p v) = a0.
+Proof.
+  revert m p.
+  induction v; intros m p.
+  - destruct m.
+    + reflexivity.
+    + contradiction (Nat.nle_succ_0 m p).
+  - destruct m.
+    + reflexivity.
+    + simpl insert.
+      change (Vnth (nat_to_fin (le_n_S (S m) (S n) p)) (Vcons a (insert a0 (le_S_n m n p) v))) with (Vnth (nat_to_fin (le_S_n (S m) (S n) (le_n_S (S m) (S n) p))) (insert a0 (le_S_n m n p) v)).
+      rewrite nat_to_fin_proof_irrelevance with (p := (le_S_n (S m) (S n) (le_n_S (S m) (S n) p))) (q := le_n_S m n (le_S_n m n p)).
+      apply IHv.
+Qed.
+
+
+Lemma fin_incl_proof_irrelevance (n m : nat) (p q : m <= n) :
+  fin_incl p = fin_incl q.
+Proof.
+  revert m p q.
+  induction n; intro m.
+  - destruct m; intros p q.
+    + reflexivity.
+    + contradiction (Nat.nle_succ_0 m p).
+  - destruct m; intros p q.
+    + reflexivity.
+    + simpl fin_incl.
+      rewrite IHn with (p := le_S_n m n p) (q := le_S_n m n q).
+      reflexivity.
+Qed.
+
+Lemma vect_proj_proof_irrelevance (A : Type) (n m : nat) (p q : m <= n) :
+  @vect_proj A n m p = @vect_proj A n m q.
+Proof.
+  revert m p q.
+  induction n; intro m.
+  - destruct m; intros p q.
+    + reflexivity.
+    + contradiction (Nat.nle_succ_0 m p).
+  - destruct m; intros p q.
+    + reflexivity.
+    + simpl vect_proj.
+      rewrite IHn with (p := le_S_n m n p) (q := le_S_n m n q).
+      reflexivity.
+Qed.
+
+Lemma nat_to_fin_incl (n m o : nat) (p : m < n) (q : n <= o) :
+  fin_incl q (nat_to_fin p) = nat_to_fin (Nat.le_trans (S m) n o p q).
+Proof.
+  revert n q m p.
+  induction o.
+  - intros n q m p.
+    contradiction (Nat.nle_succ_0 m (Nat.le_trans (S m) n 0 p q)).
+  - induction n; intro q.
+    + intros m p.
+      contradiction (Nat.nle_succ_0 m p).
+    + induction m; intro p.
+      * reflexivity.
+      * simpl.
+        apply f_equal with (f := @Succ o).
+        rewrite nat_to_fin_proof_irrelevance with (p := le_S_n (S m) o (Nat.le_trans (S (S m)) (S n) (S o) p q)) (q := Nat.le_trans (S m) n o (le_S_n (S m) n p) (le_S_n n o q)).
+        apply IHo with (q := le_S_n n o q) (p := le_S_n (S m) n p).
+Qed.
+
+(** Definition of formulas **)
+
 Inductive form : Type :=
-| free_var (x : nat)
-| bound_var (x : nat) 
-| bot
-| imp (s t : form)
-| conj (s t : form)
-| disj (s t : form)
-| for_all (s : form)
-| exist (s : form).
+  | free_var (x : nat)
+  | bound_var (x : nat) 
+  | bot
+  | imp (s t : form)
+  | conj (s t : form)
+  | disj (s t : form)
+  | for_all (s : form)
+  | exist (s : form).
+
+(* Replacing a bound variable by a given free variable *)
+
+Fixpoint unbind_rec (s : form) (x height : nat) : form :=
+  match s with
+    | free_var n => free_var n
+    | bound_var n => remove_nat height bound_var 0 (free_var x) n
+    | bot => bot
+    | imp s t => imp (unbind_rec s x height) (unbind_rec t x height)
+    | conj s t => conj (unbind_rec s x height) (unbind_rec t x height)
+    | disj s t => disj (unbind_rec s x height) (unbind_rec t x height)
+    | for_all s => for_all (unbind_rec s x (S height))
+    | exist s => exist (unbind_rec s x (S height))
+    end.
+
+Definition unbind (s : form) (x : nat) : form :=
+  unbind_rec s x 0.
+
+(** Predicate which ensures that a given free variable does not appear in a formula **)
 
 Inductive not_free_in : nat -> form -> Prop :=
   |NF_free_var (m n : nat) : m <> n -> not_free_in m (free_var n)
@@ -28,72 +463,6 @@ Inductive not_free_in : nat -> form -> Prop :=
 Inductive not_free_in_ctx : nat -> list form -> Prop :=
   |NFC_nil (x : nat) : not_free_in_ctx x []
   |NFC_l (x : nat) (s : form) (A : list form) : not_free_in x s -> not_free_in_ctx x A -> not_free_in_ctx x (s::A).
-
-(*
-Fixpoint bind_height (x height : nat) (s : form) : form :=
-  match s with
-  | free_var n => if Nat.eqb x n then bound_var height else free_var n
-  | bound_var n => bound_var n
-  | bot => bot
-  | imp s t => imp (bind_height x height s) (bind_height x height t)
-  | conj s t => conj (bind_height x height s) (bind_height x height t)
-  | disj s t => disj (bind_height x height s) (bind_height x height t)
-  | for_all s => for_all (bind_height x (S height) s)
-  | exist s => exist (bind_height x (S height) s)
-  end.
-
-Definition bind (x : nat) (s : form) : form :=
-  bind_height x 0 s.
-
-Definition my_for_all (x : nat) (s : form) : form :=
-  for_all (bind x s).
-
-Definition my_exist (x : nat) (s : form) : form :=
-  exist (bind x s).
-*)
-
-Definition unbind (s : form) (x : nat) : form :=
-  let fix aux (s : form) (x height : nat) : form :=
-  match s with
-    | free_var n => free_var n
-    | bound_var n => if Nat.eqb height n then free_var x else bound_var n
-    | bot => bot
-    | imp s t => imp (aux s x height) (aux t x height)
-    | conj s t => conj (aux s x height) (aux t x height)
-    | disj s t => disj (aux s x height) (aux t x height)
-    | for_all s => for_all (aux s x (S height))
-    | exist s => exist (aux s x (S height))
-    end
-  in aux s x 0.
-
-Print In.
-Print incl.
-
-Notation "s ~> t" := (imp s t) ( at level 51, right associativity).
-Notation neg s := ( imp s bot).
-Reserved Notation "A |- s" (at level 70).
-
-(** 2.a *)
-Inductive nd : list form -> form -> Prop :=
-  |Ass A s : (In s A) -> nd A s
-  |Exp A s : nd A bot -> nd A s
-  |Iimp A s t : nd (s::A) t -> nd A (s ~> t)
-  |Eimp A s t : nd A s -> nd A (s ~> t) -> nd A t
-  |Iconj A s t : nd A s -> nd A t -> nd A (conj s t)
-  |Econjr A s t : nd A (conj s t) -> nd A t
-  |Econjl A s t : nd A (conj s t) -> nd A s
-  |Idisjr A s t : nd A t -> nd A (disj s t)
-  |Idisjl A s t : nd A s -> nd A (disj s t)
-  |Edisj A s t u : nd A (disj s t) -> nd A (imp s u) -> nd A (imp t u) -> nd A u
-  |Ifor_all A s x : not_free_in_ctx x A -> not_free_in x s -> nd A (unbind s x) -> nd A (for_all s)
-  |Efor_all A s x : nd A (for_all s) -> nd A (unbind s x)
-  |Iexist A s x : nd A (unbind s x) -> nd A (exist s)
-  |Eexist A s t x : not_free_in_ctx x A -> not_free_in x s -> not_free_in x t -> nd A (exist s) -> nd A (imp (unbind s x) t) -> nd A t.
-
-
-Notation "A |- s" := (nd A s) ( at level 70).
-
-(* Properties of not_free_in *)
 
 Lemma NF_free_var_eq (x n : nat) :
   not_free_in x (free_var n) <-> x <> n.
@@ -247,8 +616,6 @@ Proof.
     apply NF_exist.
     assumption.
 Qed.
-
-(* Properties of not_free_in_ctx *)
 
 Lemma NFC_in (A : list form) (x : nat) (a : form) : In a A -> not_free_in_ctx x A -> not_free_in x a.
 Proof.
@@ -406,114 +773,277 @@ Proof.
   apply Nat.le_refl.
 Qed.
 
-(* Defining a function nat -> nat which swaps two integers *)
+(** Predicate which ensures that all bound variables are linked to a quantifier **)
 
-Definition exchange_nat (x y z : nat) : nat :=
-  if Nat.eqb z x then y else if Nat.eqb z y then x else z.
+Inductive is_valid : nat -> form -> Prop :=
+| Valid_free_var : forall (depth x : nat), is_valid depth (free_var x)
+| Valid_bound_var : forall (depth n : nat), n < depth -> is_valid depth (bound_var n)
+| Valid_bot : forall (depth : nat), is_valid depth bot
+| Valid_imp : forall (depth : nat) (s t : form), is_valid depth s -> is_valid depth t -> is_valid depth (imp s t)
+| Valid_conj : forall (depth : nat) (s t : form), is_valid depth s -> is_valid depth t -> is_valid depth (conj s t)
+| Valid_disj : forall (depth : nat) (s t : form), is_valid depth s -> is_valid depth t -> is_valid depth (disj s t)
+| Valid_for_all : forall (depth : nat) (s : form), is_valid (S depth) s -> is_valid depth (for_all s)
+| Valid_exist : forall (depth : nat) (s : form), is_valid (S depth) s -> is_valid depth (exist s).
 
-(*
-Lemma exchange_nat_refl (x y : nat) :
-  exchange_nat x x y = y.
+Lemma valid_bound_var_eq (depth n : nat) :
+  is_valid depth (bound_var n) -> n < depth.
 Proof.
-  unfold exchange_nat.
-  destruct (Bool.bool_dec (Nat.eqb y x) true) as [Eq | Neq].
-  + rewrite Eq.
-    apply Nat.eqb_eq.
-    rewrite Nat.eqb_sym with (x := x) (y := y).
-    assumption.
-  + apply Bool.not_true_iff_false in Neq.
-    rewrite Neq.
-    reflexivity.
-Qed.
-*)
+  remember (bound_var n) as s.
+  intro HValid.
+  destruct HValid; solve [discriminate Heqs | injection Heqs; intro Eqs; rewrite <- Eqs; assumption].
+Defined.
 
-(*
-Lemma exchange_nat_sym (x y z : nat) :
-  exchange_nat x y z = exchange_nat y x z.
+Lemma valid_imp_eq (depth : nat) (s t : form) :
+  is_valid depth (imp s t) -> is_valid depth s /\ is_valid depth t.
 Proof.
-  unfold exchange_nat.
-  destruct (Bool.bool_dec (Nat.eqb z x) true) as [Eq | Neq].
-  + rewrite Eq.
-    destruct (Bool.bool_dec (Nat.eqb z y) true) as [Eq1 | Neq1].
-    * rewrite Eq1.
-      apply eq_trans with (y := z).
-      apply eq_sym.
-      apply Nat.eqb_eq.
-      assumption.
-      apply Nat.eqb_eq.
-      assumption.
-    * apply Bool.not_true_iff_false in Neq1.
-      rewrite Neq1.
-      reflexivity.
-  + apply Bool.not_true_iff_false in Neq.
-    rewrite Neq.
-    destruct (Bool.bool_dec (Nat.eqb z y) true) as [Eq1 | Neq1].
-    * rewrite Eq1.
-      reflexivity.
-    * apply Bool.not_true_iff_false in Neq1.
-      rewrite Neq1.
-      reflexivity.
-Qed.
-*)
+  remember (imp s t) as u.
+  intro HValid.
+  destruct HValid; solve [discriminate Hequ | injection Hequ; intros Eqt Eqs; rewrite <- Eqt; rewrite <- Eqs; split; assumption]. 
+Defined.
 
-Lemma exchange_nat_l (x y : nat) :
-  exchange_nat x y x = y.
+Lemma valid_conj_eq (depth : nat) (s t : form) :
+  is_valid depth (conj s t) -> is_valid depth s /\ is_valid depth t.
 Proof.
-  unfold exchange_nat.
-  rewrite (Nat.eqb_refl x).
-  reflexivity.
-Qed.
+  remember (conj s t) as u.
+  intro HValid.
+  destruct HValid; solve [discriminate Hequ | injection Hequ; intros Eqt Eqs; rewrite <- Eqt; rewrite <- Eqs; split; assumption]. 
+Defined.
 
-Lemma exchange_nat_r (x y : nat) :
-  exchange_nat x y y = x.
+Lemma valid_disj_eq (depth : nat) (s t : form) :
+  is_valid depth (disj s t) -> is_valid depth s /\ is_valid depth t.
 Proof.
-  unfold exchange_nat.
-  destruct (Bool.bool_dec (Nat.eqb y x) true) as [Eq | Neq].
-  - rewrite Eq.
-    apply Nat.eqb_eq.
-    assumption.
-  - apply Bool.not_true_iff_false in Neq.
-    rewrite Neq.
-    rewrite (Nat.eqb_refl y).
-    reflexivity.
-Qed.
+  remember (disj s t) as u.
+  intro HValid.
+  destruct HValid; solve [discriminate Hequ | injection Hequ; intros Eqt Eqs; rewrite <- Eqt; rewrite <- Eqs; split; assumption]. 
+Defined.
 
-Lemma exchange_nat_inv (x y z : nat) :
-  exchange_nat x y (exchange_nat x y z) = z.
+Lemma valid_for_all_eq (depth : nat) (s : form) :
+  is_valid depth (for_all s) -> is_valid (S depth) s.
 Proof.
-  unfold exchange_nat.
-  destruct (Bool.bool_dec (Nat.eqb z x) true) as [Eq | Neq].
-  + rewrite Eq.
-    destruct (Bool.bool_dec (Nat.eqb y x) true) as [Eq1 | Neq1].
-    * rewrite Eq1.
-      apply eq_trans with (y := x).
-      apply Nat.eqb_eq.
-      assumption.
-      apply eq_sym.
-      apply Nat.eqb_eq.
-      assumption.
-    * apply Bool.not_true_iff_false in Neq1.
-      rewrite Neq1.
-      rewrite (Nat.eqb_refl y).
-      apply eq_sym.
-      apply Nat.eqb_eq.
-      assumption.
-  + apply Bool.not_true_iff_false in Neq.
-    rewrite Neq.
-    destruct (Bool.bool_dec (Nat.eqb z y) true) as [Eq1 | Neq1].
-    * rewrite Eq1.
-      rewrite (Nat.eqb_refl x).
-      apply eq_sym.
-      apply Nat.eqb_eq.
-      assumption.
-    * apply Bool.not_true_iff_false in Neq1.
-      rewrite Neq1.
-      rewrite Neq.
-      rewrite Neq1.
-      reflexivity.
+  remember (for_all s) as t.
+  intro HValid.
+  destruct HValid; solve [discriminate Heqt | injection Heqt; intro Eqs; rewrite <- Eqs; assumption].
+Defined.
+
+Lemma valid_exist_eq (depth : nat) (s : form) :
+  is_valid depth (exist s) -> is_valid (S depth) s.
+Proof.
+  remember (exist s) as t.
+  intro HValid.
+  destruct HValid; solve [discriminate Heqt | injection Heqt; intro Eqs; rewrite <- Eqs; assumption].
+Defined.
+
+Lemma is_valid_increasing (f : form) (depth depth' : nat) :
+  depth <= depth' -> is_valid depth f -> is_valid depth' f.
+Proof.
+  intros Hle Hvalid.
+  revert depth' Hle.
+  induction Hvalid; intros depth' Hle.
+  - apply Valid_free_var.
+  - apply Valid_bound_var.
+    apply Nat.le_trans with (m := depth).
+    + apply H.
+    + apply Hle.
+  - apply Valid_bot.
+  - apply Valid_imp.
+    + apply IHHvalid1.
+      apply Hle.
+    + apply IHHvalid2.
+      apply Hle.
+  - apply Valid_conj.
+    + apply IHHvalid1.
+      apply Hle.
+    + apply IHHvalid2.
+      apply Hle.
+  - apply Valid_disj.
+    + apply IHHvalid1.
+      apply Hle.
+    + apply IHHvalid2.
+      apply Hle.
+  - apply Valid_for_all.
+    apply IHHvalid.
+    apply le_n_S.
+    apply Hle.
+  - apply Valid_exist.
+    apply IHHvalid.
+    apply le_n_S.
+    apply Hle.
 Qed.
 
-(* Exchanging all the occurences of two variables in a formula *)
+Lemma is_valid_eventually (f : form) :
+  exists (depth : nat), is_valid depth f.
+Proof.
+  induction f.
+  - exists 0.
+    apply Valid_free_var.
+  - exists (S x).
+    apply Valid_bound_var.
+    apply Nat.le_refl.
+  - exists 0.
+    apply Valid_bot.
+  - destruct IHf1.
+    destruct IHf2.
+    exists (Nat.max x x0).
+    apply Valid_imp.
+    + apply (is_valid_increasing (Nat.le_max_l x x0) H).
+    + apply (is_valid_increasing (Nat.le_max_r x x0) H0).
+  - destruct IHf1.
+    destruct IHf2.
+    exists (Nat.max x x0).
+    apply Valid_conj.
+    + apply (is_valid_increasing (Nat.le_max_l x x0) H).
+    + apply (is_valid_increasing (Nat.le_max_r x x0) H0).
+  - destruct IHf1.
+    destruct IHf2.
+    exists (Nat.max x x0).
+    apply Valid_disj.
+    + apply (is_valid_increasing (Nat.le_max_l x x0) H).
+    + apply (is_valid_increasing (Nat.le_max_r x x0) H0).
+  - destruct IHf.
+    exists x.
+    apply Valid_for_all.
+    apply (is_valid_increasing (Nat.le_succ_diag_r x) H).
+  - destruct IHf.
+    exists x.
+    apply Valid_exist.
+    apply (is_valid_increasing (Nat.le_succ_diag_r x) H).
+Qed.
+
+Lemma valid_unbind_rec (f : form) (x depth height : nat) :
+  height <= depth -> (is_valid (S depth) f <-> is_valid depth (unbind_rec f x height)).
+Proof.
+  revert depth height.
+  induction f; intros depth height Hle; unfold unbind_rec.
+  - split; intro H; apply Valid_free_var.
+  - destruct Nat.lt_trichotomy with (n := x0) (m := height).
+    + rewrite remove_nat_lt.
+        split; intro H0; apply Valid_bound_var.
+        apply Nat.le_trans with (m := height).
+          apply H.
+          apply Hle.
+        apply Nat.le_trans with (m := height).
+          apply H.
+          apply le_S.
+          apply Hle.
+        apply H.
+    + destruct H.
+      * rewrite H.
+        rewrite remove_nat_eq.
+        split; intro H0.
+          apply Valid_free_var.
+          apply Valid_bound_var.
+          apply le_n_S.
+          apply Hle.
+      * destruct x0.
+          contradiction (Nat.nle_succ_0 height H).
+          rewrite remove_nat_gt.
+            split; intro H0; apply Valid_bound_var.
+              apply le_S_n.
+              apply (valid_bound_var_eq H0).
+              apply le_n_S.
+              apply (valid_bound_var_eq H0).
+              apply le_S_n.
+            apply H.
+  - split; intro H; apply Valid_bot.
+  - split; intro H.
+    + apply Valid_imp.
+      * apply IHf1.
+          apply Hle.
+          apply (valid_imp_eq H).
+      * apply IHf2.
+          apply Hle.
+          apply (valid_imp_eq H).
+    + apply Valid_imp.
+      * apply <- IHf1.
+          apply (valid_imp_eq H).
+          apply Hle.
+      * apply <- IHf2.
+          apply (valid_imp_eq H).
+          apply Hle.
+  - split; intro H.
+    + apply Valid_conj.
+      * apply IHf1.
+          apply Hle.
+          apply (valid_conj_eq H).
+      * apply IHf2.
+          apply Hle.
+          apply (valid_conj_eq H).
+    + apply Valid_conj.
+      * apply <- IHf1.
+          apply (valid_conj_eq H).
+          apply Hle.
+      * apply <- IHf2.
+          apply (valid_conj_eq H).
+          apply Hle.
+  - split; intro H.
+    + apply Valid_disj.
+      * apply IHf1.
+          apply Hle.
+          apply (valid_disj_eq H).
+      * apply IHf2.
+          apply Hle.
+          apply (valid_disj_eq H).
+    + apply Valid_disj.
+      * apply <- IHf1.
+          apply (valid_disj_eq H).
+          apply Hle.
+      * apply <- IHf2.
+          apply (valid_disj_eq H).
+          apply Hle.
+  - split; intro H.
+    + apply Valid_for_all.
+      apply IHf.
+      * apply le_n_S.
+        apply Hle.
+      * apply (valid_for_all_eq H).
+    + apply Valid_for_all.
+      apply <- IHf.
+      * apply (valid_for_all_eq H).
+      * apply le_n_S.
+        apply Hle.
+  - split; intro H.
+    + apply Valid_exist.
+      apply IHf.
+      * apply le_n_S.
+        apply Hle.
+      * apply (valid_exist_eq H).
+    + apply Valid_exist.
+      apply <- IHf.
+      * apply (valid_exist_eq H).
+      * apply le_n_S.
+        apply Hle.
+Qed.
+
+Inductive is_valid_ctx : nat -> list form -> Prop :=
+  | Valid_nil : forall (depth : nat), is_valid_ctx depth []
+  | Valid_cons : forall (depth : nat) (a : form) (A : list form), is_valid depth a -> is_valid_ctx depth A -> is_valid_ctx depth (a::A).
+
+Lemma valid_cons_eq (depth : nat) (a : form) (A : list form) :
+  is_valid_ctx depth (a::A) -> is_valid depth a /\ is_valid_ctx depth A.
+Proof.
+  remember (a::A) as A'.
+  intro HValid.
+  destruct HValid.
+  - discriminate HeqA'.
+  - injection HeqA'.
+    intros EqA Eqa.
+    rewrite <- EqA.
+    rewrite <- Eqa.
+    split; assumption.
+Qed.
+
+Lemma is_valid_ctx_increasing (A : list form) (depth depth' : nat) :
+  depth <= depth' -> is_valid_ctx depth A -> is_valid_ctx depth' A.
+Proof.
+  intros Hle HValid.
+  induction HValid.
+  - apply Valid_nil.
+  - apply Valid_cons.
+    + apply (is_valid_increasing Hle H).
+    + apply (IHHValid Hle).
+Qed.
+
+(** Exchanging all the occurences of two given variables in a formula **)
 
 Fixpoint exchange_vars (s : form) (x y : nat) : form :=
   match s with
@@ -527,67 +1057,6 @@ Fixpoint exchange_vars (s : form) (x y : nat) : form :=
   | exist s => exist (exchange_vars s x y)
   end.
 
-(*
-Lemma exchange_vars_refl (s : form) (x : nat) :
-  exchange_vars s x x = s.
-Proof.
-  induction s.
-  - unfold exchange_vars.
-    apply f_equal.
-    apply exchange_nat_refl.
-  - reflexivity.
-  - reflexivity.
-  - simpl exchange_vars.
-    rewrite IHs1.
-    rewrite IHs2.
-    reflexivity.
-  - simpl exchange_vars.
-    rewrite IHs1.
-    rewrite IHs2.
-    reflexivity.
-  - simpl exchange_vars.
-    rewrite IHs1.
-    rewrite IHs2.
-    reflexivity.
-  - simpl exchange_vars.
-    rewrite IHs.
-    reflexivity.
-  - simpl exchange_vars.
-    rewrite IHs.
-    reflexivity.
-Qed.
-*)
-
-(*
-Lemma exchange_vars_sym (s : form) (x y : nat) :
-  exchange_vars s x y = exchange_vars s y x.
-Proof.
-  induction s.
-  - simpl exchange_vars.
-    apply f_equal.
-    apply exchange_nat_sym.
-  - reflexivity.
-  - reflexivity.
-  - simpl exchange_vars.
-    rewrite IHs1.
-    rewrite IHs2.
-    reflexivity.
-  - simpl exchange_vars.
-    rewrite IHs1.
-    rewrite IHs2.
-    reflexivity.
-  - simpl exchange_vars.
-    rewrite IHs1.
-    rewrite IHs2.
-    reflexivity.
-  - simpl exchange_vars.
-    rewrite IHs.
-    reflexivity.
-  - simpl exchange_vars.
-    rewrite IHs.
-    reflexivity.
-Qed.
-*)
 
 Lemma exchange_vars_inv (s : form) (x y : nat) :
   exchange_vars (exchange_vars s x y) x y = s.
@@ -689,35 +1158,36 @@ Proof.
   generalize 0.
   induction s; intro height.
   - reflexivity.
-  - simpl exchange_vars.
-    destruct (Bool.bool_dec (Nat.eqb height x0) true) as [Eq | Neq].
-    + rewrite Eq.
-      reflexivity.
-    + apply Bool.not_true_iff_false in Neq.
-      rewrite Neq.
-      reflexivity.
+  - simpl.
+    generalize 0 as offset.
+    revert x0.
+    induction height; intro x0.
+    + destruct x0; intro offset; reflexivity.
+    + destruct x0; intro offset.
+      * reflexivity.
+      * apply IHheight.
   - reflexivity.
   - simpl exchange_vars.
-    unfold unbind.
+    unfold unbind_rec.
     apply f_equal2.
     + apply IHs1.
     + apply IHs2.
   - simpl exchange_vars.
-    unfold unbind.
+    unfold unbind_rec.
     apply f_equal2.
     + apply IHs1.
     + apply IHs2.
   - simpl exchange_vars.
-    unfold unbind.
+    unfold unbind_rec.
     apply f_equal2.
     + apply IHs1.
     + apply IHs2.
   - simpl exchange_vars.
-    unfold unbind.
+    unfold unbind_rec.
     apply f_equal.
     apply IHs.
   - simpl exchange_vars.
-    unfold unbind.
+    unfold unbind_rec.
     apply f_equal.
     apply IHs.
 Qed.
@@ -759,36 +1229,10 @@ Proof.
     apply IHs; apply NF_exist_eq; assumption.
 Qed.
 
-(* Exchanging the occurences of two variables in a context *)
+(** Exchanging the occurences of two given variables in a context **)
 
 Definition exchange_vars_ctx (A : list form) (x y : nat) : list form :=
   map (fun (s : form) => exchange_vars s x y) A.
-
-(*
-Lemma exchange_vars_ctx_refl (A : list form) (x : nat) :
-  exchange_vars_ctx A x x = A.
-Proof.
-  induction A.
-  - reflexivity.
-  - simpl exchange_vars_ctx.
-    apply f_equal2.
-    + apply exchange_vars_refl.
-    + assumption.
-Qed.
-*)
-
-(*
-Lemma exchange_vars_ctx_sym (A : list form) (x y : nat) :
-  exchange_vars_ctx A x y = exchange_vars_ctx A y x.
-Proof.
-  induction A.
-  - reflexivity.
-  - simpl exchange_vars_ctx.
-    apply f_equal2.
-    + apply exchange_vars_sym.
-    + assumption.
-Qed.
-*)
 
 Lemma exchange_vars_ctx_inv (A : list form) (x y : nat) :
   exchange_vars_ctx (exchange_vars_ctx A x y) x y = A.
@@ -839,6 +1283,33 @@ Proof.
     + apply IHA; apply NFC_l_eq with (s := a); assumption.
 Qed.
 
+Print In.
+Print incl.
+
+Notation "s ~> t" := (imp s t) ( at level 51, right associativity).
+Notation neg s := ( imp s bot).
+Reserved Notation "A |- s" (at level 70).
+
+(** 2.a : Defining proofs and proving weakness *)
+
+Inductive nd : list form -> form -> Prop :=
+  |Ass A s : (In s A) -> nd A s
+  |Exp A s : nd A bot -> nd A s
+  |Iimp A s t : nd (s::A) t -> nd A (s ~> t)
+  |Eimp A s t : nd A s -> nd A (s ~> t) -> nd A t
+  |Iconj A s t : nd A s -> nd A t -> nd A (conj s t)
+  |Econjr A s t : nd A (conj s t) -> nd A t
+  |Econjl A s t : nd A (conj s t) -> nd A s
+  |Idisjr A s t : nd A t -> nd A (disj s t)
+  |Idisjl A s t : nd A s -> nd A (disj s t)
+  |Edisj A s t u : nd A (disj s t) -> nd A (imp s u) -> nd A (imp t u) -> nd A u
+  |Ifor_all A s x : not_free_in_ctx x A -> not_free_in x s -> nd A (unbind s x) -> nd A (for_all s)
+  |Efor_all A s x : nd A (for_all s) -> nd A (unbind s x)
+  |Iexist A s x : nd A (unbind s x) -> nd A (exist s)
+  |Eexist A s t x : not_free_in_ctx x A -> not_free_in x s -> not_free_in x t -> nd A (exist s) -> nd A (imp (unbind s x) t) -> nd A t.
+
+
+Notation "A |- s" := (nd A s) ( at level 70).
 
 Lemma exchange_vars_proof (A : list form) (s : form) (x y : nat) :
   nd A s -> nd (exchange_vars_ctx A x y) (exchange_vars s x y).
@@ -905,7 +1376,6 @@ Proof.
     + rewrite <- exchange_vars_unbind.
       apply IHND2.
 Qed.
-
 
 Fact Weak A B s :
   A |- s -> incl A B -> B |- s.
@@ -1024,222 +1494,167 @@ Proof.
         assumption.
 Qed.
 
-(** 2.b *)
+(** 2.b : Defining Heyting algebras and proving their base properties **)
+
 Record HeytingAlgebra : Type :=
 { H : Type;
   leq : H -> H -> Prop;
   leq_refl s : leq s s;
   leq_trans s t u: (leq s t -> leq t u -> leq s u);
   bottom : H;
-  meet : H -> H -> H;
+  inf : (H -> Prop) -> H;
   impl : H -> H -> H;
-  join : H -> H -> H;
-  inf : (H -> H) -> H;
-  sup : (H -> H) -> H;
   leq_bottom u : leq bottom u;
-  leq_meet s t u : ((leq u s) /\ (leq u t)) <-> leq u (meet s t);
-  leq_impl s t u : (leq (meet s t) u) <-> leq s (impl t u);
-  leq_join s t u : ((leq s u) /\ (leq t u)) <-> leq (join s t) u;
-  leq_inf f u : (forall (s:H), leq u (f s)) <-> leq u (inf f);
-  leq_sup f u : (forall (s:H), leq (f s) u) <-> leq (sup f) u
+  leq_inf (P : H -> Prop) u : (forall (s:H), P s -> leq u s) <-> leq u (inf P);
+  leq_impl s t u : (leq (inf (finite_set [s;t])) u) <-> leq s (impl t u)
 }.
 
-(** 2.c *)
+Definition meet {HA} (s t : H HA) : H HA := inf (finite_set [s;t]).
 
-(* Implémentation de vect A n comme type des fonctions d'un ensemble fini de cardinal n dans A *)
-
-Inductive fin : nat -> Set :=
-  | Zero : forall (n : nat), fin (S n)
-  | Succ : forall (n : nat), fin n -> fin (S n).
-
-Inductive vect (A : Type) : nat -> Type :=
-  | Vnil : vect A 0
-  | Vcons : forall (n : nat), A -> vect A n -> vect A (S n).
-
-Fixpoint nat_to_fin (n m : nat) : m < n ->  fin n :=
-  match n with
-  | 0 => fun p => except ((Nat.nle_succ_0 m) p)
-  | S n => match m with
-           | 0 => fun p => Zero n
-           | S m => fun p => Succ (nat_to_fin (le_S_n (S m) n p))
-           end
-  end.
-
-Fixpoint fin_incl (n m : nat) : m <= n -> fin m -> fin n :=
-  match n with
-  | 0 => match m with
-         | 0 => fun _ t => t
-         | S m => fun p _ => except (Nat.nle_succ_0 m p)
-         end
-  | S n => match m with
-           | 0 => fun _ (t : fin 0) => match t in fin m return (match m with 0 => fin (S n) | S _ => unit end) with
-                             | Zero _ => tt
-                             | Succ _ => tt
-                             end
-           | S m => fun p t => let t := match t in fin (S m) return option (fin m) with
-                               | Zero _ => None
-                               | Succ t => Some t
-                               end in match t with
-                               | None => Zero n
-                               | Some t => Succ (fin_incl (le_S_n m n p) t)
-                               end
-           end
-  end.
-
-
-Fixpoint vect_proj (A : Type) (n m : nat) : m <= n -> vect A n -> vect A m :=
-  match n with
-  | 0 => match m with
-         | 0 => fun _ v => v
-         | S m => fun p _ => match (fin_incl p (Zero m)) in fin n0 return (match n0 with 0 => vect A (S m) | S _ => unit end) with
-                             | Zero _ => tt
-                             | Succ _ => tt
-                             end
-         end
-  | S n => match m with
-           | 0 => fun _ _ => Vnil A
-           | S m => fun p v => let (x,v) := (match v in vect _ (S n) return A * vect A n with
-                               | Vcons x v => (x,v)
-                               end) in Vcons x (vect_proj (le_S_n m n p) v)
-           end
-  end.
-
-Fixpoint Vnth (A : Type) (n : nat) (t : fin n) : vect A n -> A :=
-  match t with
-  | Zero n => fun v => match v with Vcons x _ => x end
-  | Succ t => fun v => Vnth t (match v with Vcons _ v => v end)
-  end.
-
-
-Lemma vect_proj_vnth (A : Type) (n m : nat) (p : m <= n) (t : fin m) (v : vect A n) :
-  Vnth t (vect_proj p v) = Vnth (fin_incl p t) v.
+Lemma leq_meet {HA} (s t u : H HA) :
+  (leq u s /\ leq u t) <-> leq u (meet s t).
 Proof.
-  revert m t p.
-  induction v; intros m t.
-  - destruct t; intro p; contradiction (Nat.nle_succ_0 n p).
-  - destruct t; intro p.
-    + reflexivity.
-    + apply IHv.
+  unfold meet.
+  rewrite <- leq_inf.
+  split; intro H.
+  - destruct H.
+    intros s0 H2.
+    destruct H2.
+    destruct H2.
+    + rewrite <- H2. assumption.
+    + destruct H2.
+      * rewrite <- H2. assumption.
+      * contradiction (in_nil H2).
+  - split; apply H; apply Finite_set.
+    + apply in_eq.
+    + apply in_cons.
+      apply in_eq.
 Qed.
 
-Fixpoint make_vect (A : Type) (n : nat) (x : A) : vect A n :=
-  match n with
-  | 0 => Vnil A
-  | S n => Vcons x (make_vect n x)
-  end.
+Definition sup {HA} (P : H HA -> Prop) : H HA :=
+  inf (fun_image (fun (t : H HA) => impl (inf (fun_image (fun (s : H HA) => impl s t) P)) t) (fun _ => True)).
 
-Fixpoint vect_app (A : Type) (n m : nat) (a0 : A) : m <= n -> vect A m -> vect A n :=
-  match n with
-  | 0 => match m with
-         | 0 => fun _ _ => Vnil A
-         | S m => fun (p : S m <= 0) _ => match fin_incl p (Zero m) in fin n0 return (match n0 with 0 => vect A 0 | S _ => unit end) with
-                                          | Zero _ => tt
-                                          | Succ _ => tt
-                                          end
-         end
-  | S n => match m with
-           | 0 => fun _ _ => make_vect (S n) a0
-           | S m => fun (p : S m <= S n) (v : vect A (S m)) => let (x,v') := (match v in vect _ (S m) return A * vect A m with
-                                                               | Vcons x v => (x,v)
-                                                               end) in Vcons x (vect_app a0 (le_S_n m n p) v')
-           end
-  end.
-
-Lemma vect_proj_app_inv (A : Type) (n m : nat) (a0 : A) (p : m <= n) (v : vect A m) :
-  vect_proj p (vect_app a0 p v) = v.
+Lemma leq_sup {HA} (P : H HA -> Prop) u :
+  (forall (s : H HA), P s -> leq s u) <-> leq (sup P) u.
 Proof.
-  revert m p v.
-  induction n; intros m p v.
-  - induction v.
-    + reflexivity.
-    + contradiction (Nat.nle_succ_0 n p).
-  - induction v.
-    + reflexivity.
-    + simpl.
-      apply f_equal2 with (f := @Vcons A n0).
-      * reflexivity.
-      * apply IHn.
+  split; intro H0.
+  - apply leq_trans with (t := impl (inf (fun_image (fun (s : H HA) => impl s u) P)) u).
+    + unfold sup.
+      apply leq_inf with (P := fun_image (fun (t : H HA) => impl (h:=HA) (inf (h:=HA) (fun_image (fun (s : H HA) => impl (h:=HA) s t) P)) t)
+        (fun _ : H HA => True)) (u := (inf (fun_image (fun t : H HA => impl (h:=HA) (inf (fun_image (fun (s : H HA) => impl (h:=HA) s t) P)) t)
+        (fun _ : H HA => True)))).
+      * apply leq_refl.
+      * apply Fun_image with (f := fun (t : H HA) => impl (inf (fun_image (fun (s : H HA) => impl s t) P)) t) (a := u).
+        trivial.
+    + apply leq_trans with (t := impl (impl (bottom HA) (bottom HA)) u).
+      * apply leq_impl.
+        apply leq_trans with (t := meet (impl (h:=HA) (inf (h:=HA) (fun_image (fun s : H HA => impl (h:=HA) s u) P)) u) (inf (h:=HA) (fun_image (fun s : H HA => impl (h:=HA) s u) P))).
+          apply leq_meet. split.
+            apply leq_meet with (s := impl (inf (fun_image (fun (s : H HA) => impl s u) P)) u) (t := impl (bottom HA) (bottom HA)) (u := meet (impl (inf (fun_image (fun (s : H HA) => impl s u) P)) u) (impl (bottom HA) (bottom HA))).
+              apply leq_refl.
+            apply leq_trans with (t := impl (bottom HA) (bottom HA)).
+              apply leq_meet with (s := impl (inf (fun_image (fun (s : H HA) => impl s u) P)) u) (t := impl (bottom HA) (bottom HA)) (u := meet (impl (inf (fun_image (fun (s : H HA) => impl s u) P)) u) (impl (bottom HA) (bottom HA))).
+                apply leq_refl.
+              apply leq_inf.
+              intros s H1.
+              destruct H1.
+              apply leq_impl.
+              apply leq_trans with (t := a).
+                apply leq_meet with (s := impl (bottom HA) (bottom HA)) (t := a) (u := meet (impl (bottom HA) (bottom HA)) a).
+                apply leq_refl.
+                apply (H0 a H1).
+              apply leq_impl.
+              apply leq_refl.
+      * apply leq_trans with (t := meet (impl (impl (bottom HA) (bottom HA)) u) (impl (bottom HA) (bottom HA))).
+          apply leq_meet. split.
+            apply leq_refl.
+            apply leq_impl.
+            apply leq_trans with (t := bottom HA).
+              apply leq_meet with (s := impl (impl (bottom HA) (bottom HA)) u) (t := bottom HA) (u := meet (impl (impl (bottom HA) (bottom HA)) u) (bottom HA)).
+              apply leq_refl.
+              apply leq_refl.
+            apply leq_impl.
+            apply leq_refl.
+  - intros s H1.
+    apply leq_trans with (t := sup P).
+    + unfold sup.
+      apply leq_inf.
+      intros t H2.
+      destruct H2.
+      apply leq_impl.
+      apply leq_trans with (t := meet (impl s a) s).
+      * apply leq_meet. split.
+          apply leq_trans with (t := inf (fun_image (fun (t : H HA) => impl t a) P)).
+            apply leq_meet with (s := s) (t := inf (fun_image (fun (t : H HA) => impl t a) P)) (u := meet s (inf (fun_image (fun (t : H HA) => impl t a) P))).
+            apply leq_refl.
+            apply leq_inf with (P := fun_image (fun (t : H HA) => impl t a) P) (u := inf (fun_image (fun (t : H HA) => impl t a) P)).
+              apply leq_refl.
+              apply Fun_image with (f := fun (t : H HA) => impl t a) (a := s).
+              apply H1.
+          apply leq_meet with (s := s) (t := inf (fun_image (fun (t : H HA) => impl t a) P)) (u := meet s (inf (fun_image (fun (t : H HA) => impl t a) P))).
+          apply leq_refl.
+      * apply leq_impl.
+        apply leq_refl.
+    + apply H0.
 Qed.
 
+Definition join {HA} (s t : H HA) : H HA := sup (finite_set [s;t]).
 
-(* is_valid *)
-
-Inductive is_valid : nat -> form -> Prop :=
-| Valid_free_var : forall (depth x : nat), is_valid depth (free_var x)
-| Valid_bound_var : forall (depth n : nat), n < depth -> is_valid depth (bound_var n)
-| Valid_bot : forall (depth : nat), is_valid depth bot
-| Valid_imp : forall (depth : nat) (s t : form), is_valid depth s -> is_valid depth t -> is_valid depth (imp s t)
-| Valid_conj : forall (depth : nat) (s t : form), is_valid depth s -> is_valid depth t -> is_valid depth (conj s t)
-| Valid_disj : forall (depth : nat) (s t : form), is_valid depth s -> is_valid depth t -> is_valid depth (disj s t)
-| Valid_for_all : forall (depth : nat) (s : form), is_valid (S depth) s -> is_valid depth (for_all s)
-| Valid_exist : forall (depth : nat) (s : form), is_valid (S depth) s -> is_valid depth (exist s).
-
-Lemma valid_bound_var_eq (depth n : nat) :
-  is_valid depth (bound_var n) -> n < depth.
+Lemma leq_join {HA} (s t u : H HA) :
+  ((leq s u) /\ (leq t u)) <-> leq (join s t) u.
 Proof.
-  remember (bound_var n) as s.
-  intro HValid.
-  destruct HValid; solve [discriminate Heqs | injection Heqs; intro Eqs; rewrite <- Eqs; assumption].
-Defined.
-
-Lemma valid_imp_eq (depth : nat) (s t : form) :
-  is_valid depth (imp s t) -> is_valid depth s /\ is_valid depth t.
-Proof.
-  remember (imp s t) as u.
-  intro HValid.
-  destruct HValid; solve [discriminate Hequ | injection Hequ; intros Eqt Eqs; rewrite <- Eqt; rewrite <- Eqs; split; assumption]. 
-Defined.
-
-Lemma valid_conj_eq (depth : nat) (s t : form) :
-  is_valid depth (conj s t) -> is_valid depth s /\ is_valid depth t.
-Proof.
-  remember (conj s t) as u.
-  intro HValid.
-  destruct HValid; solve [discriminate Hequ | injection Hequ; intros Eqt Eqs; rewrite <- Eqt; rewrite <- Eqs; split; assumption]. 
-Defined.
-
-Lemma valid_disj_eq (depth : nat) (s t : form) :
-  is_valid depth (disj s t) -> is_valid depth s /\ is_valid depth t.
-Proof.
-  remember (disj s t) as u.
-  intro HValid.
-  destruct HValid; solve [discriminate Hequ | injection Hequ; intros Eqt Eqs; rewrite <- Eqt; rewrite <- Eqs; split; assumption]. 
-Defined.
-
-Lemma valid_for_all_eq (depth : nat) (s : form) :
-  is_valid depth (for_all s) -> is_valid (S depth) s.
-Proof.
-  remember (for_all s) as t.
-  intro HValid.
-  destruct HValid; solve [discriminate Heqt | injection Heqt; intro Eqs; rewrite <- Eqs; assumption].
-Defined.
-
-Lemma valid_exist_eq (depth : nat) (s : form) :
-  is_valid depth (exist s) -> is_valid (S depth) s.
-Proof.
-  remember (exist s) as t.
-  intro HValid.
-  destruct HValid; solve [discriminate Heqt | injection Heqt; intro Eqs; rewrite <- Eqs; assumption].
-Defined.
-
-Inductive is_valid_ctx : nat -> list form -> Prop :=
-  | Valid_nil : forall (depth : nat), is_valid_ctx depth []
-  | Valid_cons : forall (depth : nat) (a : form) (A : list form), is_valid depth a -> is_valid_ctx depth A -> is_valid_ctx depth (a::A).
-
-Lemma valid_cons_eq (depth : nat) (a : form) (A : list form) :
-  is_valid_ctx depth (a::A) -> is_valid depth a /\ is_valid_ctx depth A.
-Proof.
-  remember (a::A) as A'.
-  intro HValid.
-  destruct HValid.
-  - discriminate HeqA'.
-  - injection HeqA'.
-    intros EqA Eqa.
-    rewrite <- EqA.
-    rewrite <- Eqa.
-    split; assumption.
+  unfold join.
+  rewrite <- leq_sup.
+  split; intro H.
+  - destruct H.
+    intros s0 H2.
+    destruct H2.
+    destruct H2.
+    + rewrite <- H2. assumption.
+    + destruct H2.
+      * rewrite <- H2. assumption.
+      * contradiction (in_nil H2).
+  - split; apply H; apply Finite_set.
+    + apply in_eq.
+    + apply in_cons.
+      apply in_eq.
 Qed.
 
+Lemma leq_impl_join {HA} (s t u : H HA) :
+  leq (join s t) (impl (meet (impl s u) (impl t u)) u).
+Proof.
+  unfold join.
+  unfold sup.
+  apply leq_trans with (t := impl (inf (fun_image (fun (s0 : H HA) => impl s0 u) (finite_set [s;t]))) u).
+  - apply leq_inf with (P := fun_image (fun t0 : H HA => impl (h:=HA) (inf (h:=HA) (fun_image (fun s0 : H HA => impl (h:=HA) s0 t0) (finite_set [s; t]))) t0) (fun _ : H HA => True)).
+    + apply leq_refl.
+    + apply Fun_image with (f := fun (t0 : H HA) => impl (inf (fun_image (fun (s0 : H HA) => impl s0 t0) (finite_set [s;t]))) t0) (a := u).
+      trivial.
+  - apply leq_impl.
+    apply leq_trans with (t := meet (impl (inf (fun_image (fun (s0 : H HA) => impl s0 u) (finite_set [s;t]))) u) (inf (fun_image (fun (s0 : H HA) => impl s0 u) (finite_set [s;t])))). 
+    + apply leq_meet.
+      split.
+      * apply leq_meet with (t := meet (impl s u) (impl t u)).
+        apply leq_refl.
+      * apply leq_trans with (t := meet (impl s u) (impl t u)).
+          apply leq_meet with (s := impl (inf (fun_image (fun (s0 : H HA) => impl s0 u) (finite_set [s; t]))) u).
+          apply leq_refl.
+          apply leq_inf.
+          intros s0 H0.
+          do 3 (destruct H0).
+            rewrite <- H0.
+            apply leq_meet with (t := impl t u).
+            apply leq_refl.
+            destruct H0.
+              rewrite <- H0.
+              apply leq_meet with (s := impl s u).
+              apply leq_refl.
+              contradiction (in_nil H0).
+    + apply leq_impl.
+      apply leq_refl.
+Qed.
+
+(** 2.c : Defining evaluation of a formula *)
 
 Fixpoint eval_rec {HA} (val : nat -> H HA) (f : form) (depth : nat) : is_valid depth f -> vect (H HA) depth -> H HA :=
   match f with
@@ -1249,58 +1664,9 @@ Fixpoint eval_rec {HA} (val : nat -> H HA) (f : form) (depth : nat) : is_valid d
   | imp s t => fun p => fun v => impl (eval_rec val (proj1 (valid_imp_eq p)) v) (eval_rec val (proj2 (valid_imp_eq p)) v)
   | conj s t => fun p => fun v => meet (eval_rec val (proj1 (valid_conj_eq p)) v) (eval_rec val (proj2 (valid_conj_eq p)) v)
   | disj s t => fun p => fun v => join (eval_rec val (proj1 (valid_disj_eq p)) v) (eval_rec val (proj2 (valid_disj_eq p)) v)
-  | for_all s => fun p => fun v => inf (fun x => eval_rec val (valid_for_all_eq p) (Vcons x v))
-  | exist s => fun p => fun v => sup (fun x => eval_rec val (valid_exist_eq p) (Vcons x v))
+  | for_all s => fun p => fun v => inf (fun_image (fun x => eval_rec val (valid_for_all_eq p) (Vcons x v)) (fun _ => True))
+  | exist s => fun p => fun v => sup (fun_image (fun x => eval_rec val (valid_exist_eq p) (Vcons x v)) (fun _ => True))
   end.
-
-Definition eval {HA} (val : nat -> H HA) (f : form) (p : is_valid 0 f) : H HA := eval_rec val p (Vnil (H HA)).
-
-
-(* Proof irrelevance dans toutes les fonctions ci-dessus *)
-
-Lemma nat_to_fin_proof_irrelevance (n m : nat) (p q : m < n) :
-  nat_to_fin p = nat_to_fin q.
-Proof.
-  revert m p q.
-  induction n; intro m.
-  - intro p.
-    contradiction (Nat.nle_succ_0 m p).
-  - induction m; intros p q.
-    + reflexivity.
-    + simpl nat_to_fin.
-      apply f_equal.
-      apply IHn.
-Qed.
-
-Lemma fin_incl_proof_irrelevance (n m : nat) (p q : m <= n) :
-  fin_incl p = fin_incl q.
-Proof.
-  revert m p q.
-  induction n; intro m.
-  - destruct m; intros p q.
-    + reflexivity.
-    + contradiction (Nat.nle_succ_0 m p).
-  - destruct m; intros p q.
-    + reflexivity.
-    + simpl fin_incl.
-      rewrite IHn with (p := le_S_n m n p) (q := le_S_n m n q).
-      reflexivity.
-Qed.
-
-Lemma vect_proj_proof_irrelevance (A : Type) (n m : nat) (p q : m <= n) :
-  @vect_proj A n m p = @vect_proj A n m q.
-Proof.
-  revert m p q.
-  induction n; intro m.
-  - destruct m; intros p q.
-    + reflexivity.
-    + contradiction (Nat.nle_succ_0 m p).
-  - destruct m; intros p q.
-    + reflexivity.
-    + simpl vect_proj.
-      rewrite IHn with (p := le_S_n m n p) (q := le_S_n m n q).
-      reflexivity.
-Qed.
 
 Lemma eval_rec_proof_irrelevance {HA} (val : nat -> H HA) (f : form) (depth : nat) (p q : is_valid depth f) :
   eval_rec val p = eval_rec val q.
@@ -1325,118 +1691,14 @@ Proof.
     + apply IHf1.
     + apply IHf2.
   - simpl eval_rec.
-    apply f_equal with (f := fun f v => inf (fun x => f (Vcons x v))).
+    apply f_equal with (f := fun f v => inf (fun_image (fun x => f (Vcons x v)) (fun _ => True))).
     apply IHf.
   - simpl eval_rec.
-    apply f_equal with (f := fun f v => sup (fun x => f (Vcons x v))).
+    apply f_equal with (f := fun f v => sup (fun_image (fun x => f (Vcons x v)) (fun _ => True))).
     apply IHf.
 Qed.
 
-Lemma is_valid_increasing (f : form) (depth depth' : nat) :
-  depth <= depth' -> is_valid depth f -> is_valid depth' f.
-Proof.
-  intros Hle Hvalid.
-  revert depth' Hle.
-  induction Hvalid; intros depth' Hle.
-  - apply Valid_free_var.
-  - apply Valid_bound_var.
-    apply Nat.le_trans with (m := depth).
-    + apply H0.
-    + apply Hle.
-  - apply Valid_bot.
-  - apply Valid_imp.
-    + apply IHHvalid1.
-      apply Hle.
-    + apply IHHvalid2.
-      apply Hle.
-  - apply Valid_conj.
-    + apply IHHvalid1.
-      apply Hle.
-    + apply IHHvalid2.
-      apply Hle.
-  - apply Valid_disj.
-    + apply IHHvalid1.
-      apply Hle.
-    + apply IHHvalid2.
-      apply Hle.
-  - apply Valid_for_all.
-    apply IHHvalid.
-    apply le_n_S.
-    apply Hle.
-  - apply Valid_exist.
-    apply IHHvalid.
-    apply le_n_S.
-    apply Hle.
-Qed.
-
-Lemma is_valid_ctx_increasing (A : list form) (depth depth' : nat) :
-  depth <= depth' -> is_valid_ctx depth A -> is_valid_ctx depth' A.
-Proof.
-  intros Hle HValid.
-  induction HValid.
-  - apply Valid_nil.
-  - apply Valid_cons.
-    + apply (is_valid_increasing Hle H0).
-    + apply (IHHValid Hle).
-Qed.
-
-Lemma is_valid_eventually (f : form) :
-  exists (depth : nat), is_valid depth f.
-Proof.
-  induction f.
-  - exists 0.
-    apply Valid_free_var.
-  - exists (S x).
-    apply Valid_bound_var.
-    apply Nat.le_refl.
-  - exists 0.
-    apply Valid_bot.
-  - destruct IHf1.
-    destruct IHf2.
-    exists (Nat.max x x0).
-    apply Valid_imp.
-    + apply (is_valid_increasing (Nat.le_max_l x x0) H0).
-    + apply (is_valid_increasing (Nat.le_max_r x x0) H1).
-  - destruct IHf1.
-    destruct IHf2.
-    exists (Nat.max x x0).
-    apply Valid_conj.
-    + apply (is_valid_increasing (Nat.le_max_l x x0) H0).
-    + apply (is_valid_increasing (Nat.le_max_r x x0) H1).
-  - destruct IHf1.
-    destruct IHf2.
-    exists (Nat.max x x0).
-    apply Valid_disj.
-    + apply (is_valid_increasing (Nat.le_max_l x x0) H0).
-    + apply (is_valid_increasing (Nat.le_max_r x x0) H1).
-  - destruct IHf.
-    exists x.
-    apply Valid_for_all.
-    apply (is_valid_increasing (Nat.le_succ_diag_r x) H0).
-  - destruct IHf.
-    exists x.
-    apply Valid_exist.
-    apply (is_valid_increasing (Nat.le_succ_diag_r x) H0).
-Qed.
-
-
-Lemma nat_to_fin_incl (n m o : nat) (p : m < n) (q : n <= o) :
-  fin_incl q (nat_to_fin p) = nat_to_fin (Nat.le_trans (S m) n o p q).
-Proof.
-  revert n q m p.
-  induction o.
-  - intros n q m p.
-    contradiction (Nat.nle_succ_0 m (Nat.le_trans (S m) n 0 p q)).
-  - induction n; intro q.
-    + intros m p.
-      contradiction (Nat.nle_succ_0 m p).
-    + induction m; intro p.
-      * reflexivity.
-      * simpl.
-        apply f_equal with (f := @Succ o).
-        rewrite nat_to_fin_proof_irrelevance with (p := le_S_n (S m) o (Nat.le_trans (S (S m)) (S n) (S o) p q)) (q := Nat.le_trans (S m) n o (le_S_n (S m) n p) (le_S_n n o q)).
-        apply IHo with (q := le_S_n n o q) (p := le_S_n (S m) n p).
-Qed.
+(* We define the equivalence relation of equivalence so that we can une antisymmetry in Heyting algebras *)
 
 Definition equivalent {HA} (u v : H HA) : Prop := leq u v /\ leq v u.
 
@@ -1519,61 +1781,59 @@ Proof.
       * apply Ht.
 Qed.
 
-Lemma equivalent_inf {HA} (f f' : H HA -> H HA) :
-  (forall (s : H HA), equivalent (f s) (f' s)) -> equivalent (inf f) (inf f').
+Lemma equivalent_inf {HA} (f g : H HA -> H HA) (P : H HA -> Prop) :
+  (forall (s : H HA), P s -> equivalent (f s) (g s)) -> equivalent (inf (fun_image f P)) (inf (fun_image g P)).
 Proof.
   intro Hs.
   split.
   - apply leq_inf.
-    intro s.
-    apply leq_trans with (t := f s).
-    + apply leq_inf.
-      apply leq_refl.
+    intros s Hg.
+    destruct Hg.
+    apply leq_trans with (t := f a).
+    + apply leq_inf with (P := fun_image f P).
+      * apply leq_refl.
+      * apply Fun_image.
+        apply H0.
     + apply Hs.
+      apply H0.
   - apply leq_inf.
-    intro s.
-    apply leq_trans with (t := f' s).
-    + apply leq_inf.
-      apply leq_refl.
+    intros s Hg.
+    destruct Hg.
+    apply leq_trans with (t := g a).
+    + apply leq_inf with (P := fun_image g P).
+      * apply leq_refl.
+      * apply Fun_image.
+        apply H0.
     + apply Hs.
+      apply H0.
 Qed.
 
-Lemma equivalent_sup {HA} (f f' : H HA -> H HA) :
-  (forall (s : H HA), equivalent (f s) (f' s)) -> equivalent (sup f) (sup f').
+Lemma equivalent_sup {HA} (f g : H HA -> H HA) (P : H HA -> Prop) :
+  (forall (s : H HA), P s -> equivalent (f s) (g s)) -> equivalent (sup (fun_image f P)) (sup (fun_image g P)).
 Proof.
   intro Hs.
   split.
   - apply leq_sup.
-    intro s.
-    apply leq_trans with (t := f' s).
+    intros s Hg.
+    destruct Hg.
+    apply leq_trans with (t := g a).
     + apply Hs.
-    + apply leq_sup.
-      apply leq_refl.
+      apply H0.
+    + apply leq_sup with (P := fun_image g P).
+      * apply leq_refl.
+      * apply Fun_image.
+        apply H0.
   - apply leq_sup.
-    intro s.
-    apply leq_trans with (t := f s).
+    intros s Hg.
+    destruct Hg.
+    apply leq_trans with (t := f a).
     + apply Hs.
-    + apply leq_sup.
-      apply leq_refl.
+      apply H0.
+    + apply leq_sup with (P := fun_image f P).
+      * apply leq_refl.
+      * apply Fun_image.
+        apply H0.
 Qed.
-(*
-Proof.
-  intro Hs.
-  split.
-  - apply leq_sup.
-    destruct ((proj2 (leq_sup f (sup f))) (leq_refl (sup f))).
-    exists x.
-    apply leq_trans with (t := f x).
-    + apply H0.
-    + apply Hs.
-  - apply leq_sup.
-    destruct ((proj2 (leq_sup f' (sup f'))) (leq_refl (sup f'))).
-    exists x.
-    apply leq_trans with (t := f' x).
-    + apply H0.
-    + apply Hs.
-Qed.
-*)
 
 Lemma eval_rec_vect_proj {HA} (val : nat -> H HA) (f : form) (depth depth' : nat) (p : depth <= depth') (q : is_valid depth f) (v : vect (H HA) depth') :
   equivalent (eval_rec val (is_valid_increasing p q) v) (eval_rec val q (vect_proj p v)).
@@ -1602,18 +1862,20 @@ Proof.
     + rewrite eval_rec_proof_irrelevance with (p := proj2 (valid_disj_eq (is_valid_increasing p q))) (q := is_valid_increasing p (proj2 (valid_disj_eq q))).
       apply IHf2 with (p := p) (q := proj2 (valid_disj_eq q)).
   - apply equivalent_inf.
-    intro s.
+    intros s _.
     rewrite eval_rec_proof_irrelevance with (p := valid_for_all_eq (is_valid_increasing p q)) (q := is_valid_increasing (le_n_S depth depth' p) (valid_for_all_eq q)).
     rewrite vect_proj_proof_irrelevance with (p := p) (q := le_S_n depth depth' (le_n_S depth depth' p)).
     change (Vcons s (vect_proj (le_S_n depth depth' (le_n_S depth depth' p)) v)) with (vect_proj (le_n_S depth depth' p) (Vcons s v)).
     apply IHf with (p := le_n_S depth depth' p) (q := valid_for_all_eq q).
   - apply equivalent_sup.
-    intro s.
+    intros s _.
     rewrite eval_rec_proof_irrelevance with (p := valid_exist_eq (is_valid_increasing p q)) (q := is_valid_increasing (le_n_S depth depth' p) (valid_exist_eq q)).
     rewrite vect_proj_proof_irrelevance with (p := p) (q := le_S_n depth depth' (le_n_S depth depth' p)).
     change (Vcons s (vect_proj (le_S_n depth depth' (le_n_S depth depth' p)) v)) with (vect_proj (le_n_S depth depth' p) (Vcons s v)).
     apply IHf with (p := le_n_S depth depth' p) (q := valid_exist_eq q).
 Qed.
+
+(** 2.d We define the equivalent of the function Meet_list **)
 
 Fixpoint Meet_valid_ctx {HA} (val : nat -> H HA) (A : list form) (depth : nat) : is_valid_ctx depth A -> vect (H HA) depth -> H HA :=
   match A with
@@ -1647,12 +1909,145 @@ Proof.
       apply IHA.
 Qed.
 
-Lemma nd_soundHA_aux (HA : HeytingAlgebra) (val : nat -> H HA) (A : list form) (s : form) (depth : nat) (p : is_valid_ctx depth A) (q : is_valid depth s) (v : vect (H HA) depth) :
+Lemma eval_rec_change_val HA (val : nat -> H HA) (f : form) (depth : nat) (p : is_valid depth f) (x : nat) (u : H HA) :
+  not_free_in x f -> eval_rec val p = eval_rec (change_val val x u) p.
+Proof.
+  intro NF.
+  revert depth p.
+  induction NF; intros depth p.
+  - simpl.
+    unfold change_val.
+    rewrite ((proj2 (Nat.eqb_neq m n)) H0).
+    reflexivity.
+  - reflexivity.
+  - reflexivity.
+  - simpl.
+    rewrite <- IHNF1.
+    rewrite <- IHNF2.
+    reflexivity.
+  - simpl.
+    rewrite <- IHNF1.
+    rewrite <- IHNF2.
+    reflexivity.
+  - simpl.
+    rewrite <- IHNF1.
+    rewrite <- IHNF2.
+    reflexivity.
+  - simpl.
+    rewrite IHNF.
+    reflexivity.
+  - simpl.
+    rewrite IHNF.
+    reflexivity.
+Qed.
+
+Lemma Meet_valid_ctx_change_val HA (val : nat -> H HA) (A : list form) (depth : nat) (p : is_valid_ctx depth A) (x : nat) (u : H HA) :
+  not_free_in_ctx x A -> Meet_valid_ctx val p = Meet_valid_ctx (change_val val x u) p.
+Proof.
+  intro H.
+  induction H.
+  - reflexivity.
+  - simpl.
+    rewrite <- eval_rec_change_val.
+    rewrite <- IHnot_free_in_ctx.
+    reflexivity.
+    apply H0.
+Qed.
+
+Lemma eval_rec_unbind HA (val : nat -> H HA) (f : form) (depth : nat) (p : is_valid (S depth) f) (v : vect (H HA) depth) (x : nat) :
+  equivalent (eval_rec val (proj1 (valid_unbind_rec f x (Nat.le_0_l depth)) p) v) (eval_rec val p (Vcons (val x) v)).
+Proof.
+  rewrite (f_equal (eval_rec val p) (match v as v0 in (vect _ n0) return (Vcons (val x) v0 = insert (val x) (Nat.le_0_l n0) v0) with
+                                                       | Vnil _ => eq_refl
+                                                       | @Vcons _ n0 a v0 => eq_refl
+                                                       end)).
+  generalize (Nat.le_0_l depth) as q.
+  generalize 0 as height.
+  revert depth p v.
+  induction f; intros depth p v height q.
+  - split; apply leq_refl.
+  - generalize (proj1 (valid_unbind_rec (bound_var x0) x q) p) as r.
+    destruct Nat.lt_trichotomy with (n := x0) (m := height); simpl unbind_rec.
+    + simpl unbind_rec.
+      rewrite remove_nat_lt with (x := height) (f := bound_var) (default := free_var x) (y := x0).
+      * intro r.
+        simpl eval_rec.
+        rewrite nat_to_fin_proof_irrelevance with (p := valid_bound_var_eq r) (q := Nat.le_trans (S x0) height depth H0 q).
+        change (match x0 as m0 return (m0 < S depth -> fin (S depth)) with
+                | 0 => fun _ : 0 < S depth => Zero depth
+                | S m => fun p0 : S m < S depth => Succ (nat_to_fin (n:=depth) (m:=m) (le_S_n (S m) depth p0))
+                end (valid_bound_var_eq p)) with (nat_to_fin (valid_bound_var_eq p)).
+        rewrite nat_to_fin_proof_irrelevance with (p := valid_bound_var_eq p) (q := le_S (S x0) depth (Nat.le_trans (S x0) height depth H0 q)).
+        rewrite insert_vnth_lt.
+        split; apply leq_refl.
+      * apply H0.
+    + destruct H0.
+      * revert p.
+        rewrite H0.
+        rewrite remove_nat_eq.
+        intros p r.
+        simpl eval_rec.
+        change (match height as m0 return (m0 < S depth -> fin (S depth)) with
+                | 0 => fun _ : 0 < S depth => Zero depth
+                | S m => fun p0 : S m < S depth => Succ (nat_to_fin (n:=depth) (m:=m) (le_S_n (S m) depth p0))
+                end (valid_bound_var_eq p)) with (nat_to_fin (valid_bound_var_eq p)).
+        rewrite nat_to_fin_proof_irrelevance with (p := valid_bound_var_eq p) (q := le_n_S height depth q).
+        rewrite insert_vnth_eq.
+        split; apply leq_refl.
+      * destruct x0. contradiction (Nat.nle_succ_0 height H0).
+        rewrite remove_nat_gt with (x := height) (f := bound_var) (default := free_var x) (y := x0).
+          intro r.
+          change (eval_rec val p (insert (val x) q v)) with (Vnth (nat_to_fin (valid_bound_var_eq p)) (insert (val x) q v)).
+          simpl eval_rec.
+          rewrite nat_to_fin_proof_irrelevance with (p := valid_bound_var_eq p) (q := le_n_S (S x0) depth (valid_bound_var_eq r)).
+          rewrite insert_proof_irrelevance with (p := q) (q := Nat.le_trans height (S x0) depth (le_S height x0 (le_S_n height x0 H0)) (valid_bound_var_eq r)).
+          rewrite insert_vnth_gt.
+          split; apply leq_refl.
+          apply le_S_n.
+          apply H0.
+  - split; apply leq_refl.
+  - simpl.
+    apply equivalent_impl.
+    + rewrite eval_rec_proof_irrelevance with (p := proj1 (valid_imp_eq (proj1 (valid_unbind_rec (imp f1 f2) x q) p))) (q := proj1 (valid_unbind_rec f1 x q) (proj1 (valid_imp_eq p))).
+      apply IHf1.
+    + rewrite eval_rec_proof_irrelevance with (p := proj2 (valid_imp_eq (proj1 (valid_unbind_rec (imp f1 f2) x q) p))) (q := proj1 (valid_unbind_rec f2 x q) (proj2 (valid_imp_eq p))).
+      apply IHf2.
+  - simpl.
+    apply equivalent_meet.
+    + rewrite eval_rec_proof_irrelevance with (p := proj1 (valid_conj_eq (proj1 (valid_unbind_rec (conj f1 f2) x q) p))) (q := proj1 (valid_unbind_rec f1 x q) (proj1 (valid_conj_eq p))).
+      apply IHf1.
+    + rewrite eval_rec_proof_irrelevance with (p := proj2 (valid_conj_eq (proj1 (valid_unbind_rec (conj f1 f2) x q) p))) (q := proj1 (valid_unbind_rec f2 x q) (proj2 (valid_conj_eq p))).
+      apply IHf2.
+  - simpl.
+    apply equivalent_join.
+    + rewrite eval_rec_proof_irrelevance with (p := proj1 (valid_disj_eq (proj1 (valid_unbind_rec (disj f1 f2) x q) p))) (q := proj1 (valid_unbind_rec f1 x q) (proj1 (valid_disj_eq p))).
+      apply IHf1.
+    + rewrite eval_rec_proof_irrelevance with (p := proj2 (valid_disj_eq (proj1 (valid_unbind_rec (disj f1 f2) x q) p))) (q := proj1 (valid_unbind_rec f2 x q) (proj2 (valid_disj_eq p))).
+      apply IHf2.
+  - simpl.
+    apply equivalent_inf.
+    intros s _.
+    rewrite insert_proof_irrelevance with (p := q) (q := le_S_n height depth (le_n_S height depth q)).
+    change (Vcons s (insert (val x) q v)) with (insert (val x) (le_n_S height depth q) (Vcons s v)).
+    rewrite eval_rec_proof_irrelevance with (p := valid_for_all_eq (proj1 (valid_unbind_rec (for_all f) x q) p)) (q := proj1 (valid_unbind_rec f x (le_n_S height depth q)) (valid_for_all_eq p)).
+    apply IHf.
+  - simpl.
+    apply equivalent_sup.
+    intros s _.
+    rewrite insert_proof_irrelevance with (p := q) (q := le_S_n height depth (le_n_S height depth q)).
+    change (Vcons s (insert (val x) q v)) with (insert (val x) (le_n_S height depth q) (Vcons s v)).
+    rewrite eval_rec_proof_irrelevance with (p := valid_exist_eq (proj1 (valid_unbind_rec (exist f) x q) p)) (q := proj1 (valid_unbind_rec f x (le_n_S height depth q)) (valid_exist_eq p)).
+    apply IHf.
+Qed.
+
+(** 2.e Proving soundness of Heyting semantics **)
+
+Lemma nd_soundHA_rec HA (val : nat -> H HA) (A : list form) (s : form) (depth : nat) (p : is_valid_ctx depth A) (q : is_valid depth s) (v : vect (H HA) depth) :
   nd A s -> leq (Meet_valid_ctx val p v) (eval_rec val q v).
 Proof.
   intro ND.
-  revert depth p q v.
-  induction ND; intros depth p q v.
+  revert val depth p q v.
+  induction ND; intros val depth p q v.
   - induction A.
     + contradiction (in_nil H0).
     + destruct H0; simpl Meet_valid_ctx.
@@ -1701,259 +2096,210 @@ Proof.
       * apply eval_rec_vect_proj.
       * rewrite vect_proj_app_inv.
         apply leq_refl.
-  - 
-
-(** 2.d *)
-Fixpoint Meet_list {HA} (val : nat -> H HA) (l : list form) :=
-  match l with
-  | nil => impl (bottom HA) (bottom HA)
-  | h::t => meet (eval val h) (Meet_list val t)
-  end.
-
-(** 2.e *)
-Definition hent HA val A s := (@Meet_list HA val A) <= (@eval HA val s).
-
-Lemma nd_soundHA HA val A s : nd A s -> @hent HA val A s.
-Proof.
-  intro H. induction H.
-  - induction A. 
-    + apply in_nil in H0. contradiction.
-    + destruct H0.
-      * unfold hent. simpl Meet_list. rewrite H0.
-        apply (leq_meet (eval val s) (Meet_list val A) (meet (h:=HA) (eval val s) (Meet_list val A))).
-        apply leq_refl.
-      * unfold hent. simpl Meet_list.
-        apply leq_trans with (t := Meet_list val A).
-        apply (leq_meet (eval val a) (Meet_list val A) (meet (h:=HA) (eval val a) (Meet_list val A))).
-        apply leq_refl.
-        apply IHA. assumption.
-  - unfold hent. apply leq_trans with (t := bottom HA).
-    + assumption.
-    + apply leq_bottom.
-  - unfold hent. simpl eval.
-    apply leq_impl.
-    unfold hent in IHnd.
-    simpl Meet_list in IHnd.
-    apply leq_trans with (t := meet (h:=HA) (eval val s) (Meet_list val A)).
-    + apply leq_meet. split;
-      apply (leq_meet (Meet_list val A) (eval val s) (meet (h:=HA) (Meet_list val A) (eval val s)));
+  - simpl eval_rec.
+    apply leq_meet.
+    split.
+    + apply IHND1.
+    + apply IHND2.
+  - destruct (is_valid_eventually s) as (depth',r).
+    rewrite <- vect_proj_app_inv with (a0 := bottom HA) (p := Nat.le_max_l depth depth') (v := v).
+    apply leq_trans with (t :=  Meet_valid_ctx val (is_valid_ctx_increasing (Nat.le_max_l depth depth') p) (vect_app (bottom HA) (Nat.le_max_l depth depth') v)).
+      + apply Meet_valid_ctx_vect_proj.
+      + apply leq_trans with (t := eval_rec val (is_valid_increasing (Nat.le_max_l depth depth') q) (vect_app (bottom HA) (Nat.le_max_l depth depth') v)).
+        * apply leq_meet with (s := eval_rec val (is_valid_increasing (Nat.le_max_r depth depth') r) (vect_app (bottom HA) (Nat.le_max_l depth depth') v)) (t := eval_rec val (is_valid_increasing (Nat.le_max_l depth depth') q) (vect_app (bottom HA) (Nat.le_max_l depth depth') v)).
+          rewrite eval_rec_proof_irrelevance with (p := is_valid_increasing (Nat.le_max_r depth depth') r) (q := proj1 (valid_conj_eq (Valid_conj (is_valid_increasing (Nat.le_max_r depth depth') r) (is_valid_increasing (Nat.le_max_l depth depth') q)))).
+          rewrite eval_rec_proof_irrelevance with (p := is_valid_increasing (Nat.le_max_l depth depth') q) (q := proj2 (valid_conj_eq (Valid_conj (is_valid_increasing (Nat.le_max_r depth depth') r) (is_valid_increasing (Nat.le_max_l depth depth') q)))).
+          apply IHND.
+        * apply eval_rec_vect_proj.
+  - destruct (is_valid_eventually t) as (depth',r).
+    rewrite <- vect_proj_app_inv with (a0 := bottom HA) (p := Nat.le_max_l depth depth') (v := v).
+    apply leq_trans with (t :=  Meet_valid_ctx val (is_valid_ctx_increasing (Nat.le_max_l depth depth') p) (vect_app (bottom HA) (Nat.le_max_l depth depth') v)).
+      + apply Meet_valid_ctx_vect_proj.
+      + apply leq_trans with (t := eval_rec val (is_valid_increasing (Nat.le_max_l depth depth') q) (vect_app (bottom HA) (Nat.le_max_l depth depth') v)).
+        * apply leq_meet with (t := eval_rec val (is_valid_increasing (Nat.le_max_r depth depth') r) (vect_app (bottom HA) (Nat.le_max_l depth depth') v)) (s := eval_rec val (is_valid_increasing (Nat.le_max_l depth depth') q) (vect_app (bottom HA) (Nat.le_max_l depth depth') v)).
+          rewrite eval_rec_proof_irrelevance with (p := is_valid_increasing (Nat.le_max_r depth depth') r) (q := proj2 (valid_conj_eq (Valid_conj (is_valid_increasing (Nat.le_max_l depth depth') q) (is_valid_increasing (Nat.le_max_r depth depth') r)))).
+          rewrite eval_rec_proof_irrelevance with (p := is_valid_increasing (Nat.le_max_l depth depth') q) (q := proj1 (valid_conj_eq (Valid_conj (is_valid_increasing (Nat.le_max_l depth depth') q) (is_valid_increasing (Nat.le_max_r depth depth') r)))).
+          apply IHND.
+        * apply eval_rec_vect_proj.
+  - apply leq_trans with (t := eval_rec val (proj2 (valid_disj_eq q)) v).
+    + apply IHND.
+    + simpl eval_rec.
+      apply leq_join with (s := eval_rec val (proj1 (valid_disj_eq q)) v).
       apply leq_refl.
-    + assumption.
-  - unfold hent.
-    apply leq_trans with (t := meet (h:=HA) (Meet_list val A) (eval val s)).
-    + apply leq_meet. split.
-      * apply leq_refl.
-      * assumption.
-    + apply leq_impl. assumption.
-  - apply leq_meet. split; assumption.
-  - apply leq_meet in IHnd. destruct IHnd. assumption.
-  - apply leq_meet in IHnd. destruct IHnd. assumption.
+  - apply leq_trans with (t := eval_rec val (proj1 (valid_disj_eq q)) v).
+    + apply IHND.
+    + simpl eval_rec.
+      apply leq_join with (t := eval_rec val (proj2 (valid_disj_eq q)) v).
+      apply leq_refl.
+  - destruct (is_valid_eventually (disj s t)) as (depth',r).
+    rewrite <- vect_proj_app_inv with (a0 := bottom HA) (p := Nat.le_max_l depth depth') (v := v).
+    apply leq_trans with (t :=  Meet_valid_ctx val (is_valid_ctx_increasing (Nat.le_max_l depth depth') p) (vect_app (bottom HA) (Nat.le_max_l depth depth') v)).
+      + apply Meet_valid_ctx_vect_proj.
+      + apply leq_trans with (t := eval_rec val (is_valid_increasing (Nat.le_max_l depth depth') q) (vect_app (bottom HA) (Nat.le_max_l depth depth') v)).
+        * apply leq_trans with (t := meet
+                                      (impl 
+                                        (meet 
+                                          (impl
+                                             (eval_rec val (proj1 (valid_disj_eq (is_valid_increasing (Nat.le_max_r depth depth') r))) (vect_app (bottom HA) (Nat.le_max_l depth depth') v))
+                                             (eval_rec val (is_valid_increasing (Nat.le_max_l depth depth') q) (vect_app (bottom HA) (Nat.le_max_l depth depth') v))
+                                          )
+                                          (impl
+                                             (eval_rec val (proj2 (valid_disj_eq (is_valid_increasing (Nat.le_max_r depth depth') r))) (vect_app (bottom HA) (Nat.le_max_l depth depth') v))
+                                             (eval_rec val (is_valid_increasing (Nat.le_max_l depth depth') q) (vect_app (bottom HA) (Nat.le_max_l depth depth') v))
+                                          )
+                                        )
+                                        (eval_rec val (is_valid_increasing (Nat.le_max_l depth depth') q) (vect_app (bottom HA) (Nat.le_max_l depth depth') v))
+                                      )
+                                      (meet
+                                        (impl
+                                          (eval_rec val (proj1 (valid_disj_eq (is_valid_increasing (Nat.le_max_r depth depth') r))) (vect_app (bottom HA) (Nat.le_max_l depth depth') v))
+                                          (eval_rec val (is_valid_increasing (Nat.le_max_l depth depth') q) (vect_app (bottom HA) (Nat.le_max_l depth depth') v))
+                                        )
+                                        (impl
+                                           (eval_rec val (proj2 (valid_disj_eq (is_valid_increasing (Nat.le_max_r depth depth') r))) (vect_app (bottom HA) (Nat.le_max_l depth depth') v))
+                                           (eval_rec val (is_valid_increasing (Nat.le_max_l depth depth') q) (vect_app (bottom HA) (Nat.le_max_l depth depth') v))
+                                        )
+                                      )
+                            ).
+            apply leq_meet.
+            split.
+              apply leq_trans with (t := eval_rec val (is_valid_increasing (Nat.le_max_r depth depth') r) (vect_app (bottom HA) (Nat.le_max_l depth depth') v)).
+                apply IHND1.
+                apply leq_impl_join.
+              apply leq_meet.
+              split.
+                rewrite eval_rec_proof_irrelevance with (p := proj1 (valid_disj_eq (is_valid_increasing (Nat.le_max_r depth depth') r))) (q := proj1 (valid_imp_eq (Valid_imp (proj1 (valid_disj_eq (is_valid_increasing (Nat.le_max_r depth depth') r))) (is_valid_increasing (Nat.le_max_l depth depth') q)))).
+                rewrite eval_rec_proof_irrelevance with (p := is_valid_increasing (Nat.le_max_l depth depth') q) (q := proj2 (valid_imp_eq (Valid_imp (proj1 (valid_disj_eq (is_valid_increasing (Nat.le_max_r depth depth') r))) (is_valid_increasing (Nat.le_max_l depth depth') q)))).
+                apply IHND2.
+                rewrite eval_rec_proof_irrelevance with (p := proj2 (valid_disj_eq (is_valid_increasing (Nat.le_max_r depth depth') r))) (q := proj1 (valid_imp_eq (Valid_imp (proj2 (valid_disj_eq (is_valid_increasing (Nat.le_max_r depth depth') r))) (is_valid_increasing (Nat.le_max_l depth depth') q)))).
+                rewrite eval_rec_proof_irrelevance with (p := is_valid_increasing (Nat.le_max_l depth depth') q) (q := proj2 (valid_imp_eq (Valid_imp (proj2 (valid_disj_eq (is_valid_increasing (Nat.le_max_r depth depth') r))) (is_valid_increasing (Nat.le_max_l depth depth') q)))).
+                apply IHND3.
+            apply leq_impl.
+            apply leq_refl.
+        * apply eval_rec_vect_proj.
+  - simpl eval_rec.
+    apply leq_inf.
+    intros s0 H2.
+    destruct H2.
+    rewrite <- change_val_refl with (f := val) (x := x) (a := a).
+    rewrite eval_rec_change_val with (x := x) (u := a).
+    rewrite Meet_valid_ctx_change_val with (x := x) (u := a).
+    apply leq_trans with (t := eval_rec (change_val val x a) (proj1 (valid_unbind_rec s x (Nat.le_0_l depth)) (valid_for_all_eq q)) v).
+    + apply IHND.
+    + apply eval_rec_unbind.
+    + apply H0.
+    + apply H1.
+  - apply leq_trans with (t := eval_rec val (Valid_for_all (proj2 (valid_unbind_rec s x (Nat.le_0_l depth)) q)) v).
+    + apply IHND.
+    + apply leq_trans with (t := eval_rec val (proj2 (valid_unbind_rec s x (Nat.le_0_l depth)) q) (Vcons (val x) v)).
+      * apply leq_inf with (P := fun_image (fun (u : H HA) => eval_rec val (proj2 (valid_unbind_rec s x (Nat.le_0_l depth)) q) (Vcons u v)) (fun _ => True)).
+          apply leq_refl.
+          apply Fun_image with (a := val x).
+          trivial.
+      * rewrite eval_rec_proof_irrelevance with (p := q) (q := (proj1 (valid_unbind_rec s x (Nat.le_0_l depth)) (proj2 (valid_unbind_rec s x (Nat.le_0_l depth)) q))).
+        apply eval_rec_unbind.
+  - apply leq_trans with (t := eval_rec val (proj1 (valid_unbind_rec s x (Nat.le_0_l depth)) (valid_exist_eq q)) v).
+    + apply IHND.
+    + apply leq_trans with (t := eval_rec val (valid_exist_eq q) (Vcons (val x) v)).
+      * apply eval_rec_unbind.
+      * apply leq_sup with (P := fun_image (fun (u : H HA) => eval_rec val (valid_exist_eq q) (Vcons u v)) (fun _ => True)).
+          apply leq_refl.
+          apply Fun_image with (a := val x).
+          trivial.
+  - destruct (is_valid_eventually (exist s)) as (depth',r).
+    rewrite <- vect_proj_app_inv with (a0 := bottom HA) (p := Nat.le_max_l depth depth') (v := v).
+    apply leq_trans with (t :=  Meet_valid_ctx val (is_valid_ctx_increasing (Nat.le_max_l depth depth') p) (vect_app (bottom HA) (Nat.le_max_l depth depth') v)).
+      + apply Meet_valid_ctx_vect_proj.
+      + apply leq_trans with (t := eval_rec val (is_valid_increasing (Nat.le_max_l depth depth') q) (vect_app (bottom HA) (Nat.le_max_l depth depth') v)).
+        * apply leq_trans with (t := meet
+                                      (eval_rec val (is_valid_increasing (Nat.le_max_r depth depth') r) (vect_app (bottom HA) (Nat.le_max_l depth depth') v))
+                                      (Meet_valid_ctx val (is_valid_ctx_increasing (Nat.le_max_l depth depth') p) (vect_app (bottom HA) (Nat.le_max_l depth depth') v))
+                               ).
+            apply leq_meet.
+            split.
+              apply IHND1.
+              apply leq_refl.
+            apply leq_impl.
+            apply (proj1 (leq_sup (fun_image (fun x0 : H HA => eval_rec val (valid_exist_eq (is_valid_increasing (Nat.le_max_r depth depth') r)) (Vcons x0 (vect_app (bottom HA) (Nat.le_max_l depth depth') v))) (fun _ : H HA => True)) (impl (h:=HA) (Meet_valid_ctx val (is_valid_ctx_increasing (Nat.le_max_l depth depth') p) (vect_app (bottom HA) (Nat.le_max_l depth depth') v)) (eval_rec val (is_valid_increasing (Nat.le_max_l depth depth') q) (vect_app (bottom HA) (Nat.le_max_l depth depth') v))))).
+            intros s0 H.
+            destruct H.
+            apply leq_impl.
+            apply leq_trans with (t := meet (Meet_valid_ctx val (is_valid_ctx_increasing (Nat.le_max_l depth depth') p) (vect_app (bottom HA) (Nat.le_max_l depth depth') v)) (eval_rec val (valid_exist_eq (is_valid_increasing (Nat.le_max_r depth depth') r)) (Vcons a (vect_app (bottom HA) (Nat.le_max_l depth depth') v)))).
+              apply leq_meet.
+              split.
+                apply leq_meet with (s := eval_rec val (valid_exist_eq (is_valid_increasing (Nat.le_max_r depth depth') r)) (Vcons a (vect_app (bottom HA) (Nat.le_max_l depth depth') v))).
+                apply leq_refl.
+                apply leq_meet with (t := Meet_valid_ctx val (is_valid_ctx_increasing (Nat.le_max_l depth depth') p) (vect_app (bottom HA) (Nat.le_max_l depth depth') v)).
+                apply leq_refl.
+              apply leq_impl.
+              rewrite <- change_val_refl with (f := val) (x := x) (a := a).
+              rewrite Meet_valid_ctx_change_val with (val := val) (x := x) (u := a).
+              rewrite eval_rec_change_val with (val := val) (x := x) (u := a).
+              rewrite eval_rec_change_val with (val := val) (x := x) (u := a).
+              apply leq_trans with (t := impl (h:=HA) (eval_rec (change_val val x a) (proj1 (valid_unbind_rec s x (Nat.le_0_l (Nat.max depth depth'))) (valid_exist_eq (is_valid_increasing (Nat.le_max_r depth depth') r))) (vect_app (bottom HA) (Nat.le_max_l depth depth') v)) (eval_rec (change_val val x a) (is_valid_increasing (Nat.le_max_l depth depth') q) (vect_app (bottom HA) (Nat.le_max_l depth depth') v))).
+                rewrite eval_rec_proof_irrelevance with (p := proj1 (valid_unbind_rec s x (Nat.le_0_l (Nat.max depth depth')))
+           (valid_exist_eq (is_valid_increasing (Nat.le_max_r depth depth') r))) (q := proj1 (valid_imp_eq (Valid_imp (proj1 (valid_unbind_rec s x (Nat.le_0_l (Nat.max depth depth')))
+           (valid_exist_eq (is_valid_increasing (Nat.le_max_r depth depth') r))) (is_valid_increasing (Nat.le_max_l depth depth') q)))).
+                rewrite eval_rec_proof_irrelevance with (p := is_valid_increasing (Nat.le_max_l depth depth') q) (q := proj2 (valid_imp_eq (Valid_imp (proj1 (valid_unbind_rec s x (Nat.le_0_l (Nat.max depth depth')))
+           (valid_exist_eq (is_valid_increasing (Nat.le_max_r depth depth') r))) (is_valid_increasing (Nat.le_max_l depth depth') q)))).
+                apply IHND2.
+                apply equivalent_impl.
+                  split; apply eval_rec_unbind.
+                  split; apply leq_refl.
+              apply H2.
+              apply H1.
+              apply H0.
+      * apply eval_rec_vect_proj.
 Qed.
 
-(** 2.f *)
+(** We now harmonize the notations to match the normal version of this exercise **)
 
-Fixpoint revert A s :=
+Record valid_form : Type :=
+{
+  f : form;
+  proof : is_valid 0 f
+}.
+
+Definition eval {HA} (val : nat -> H HA) (s : valid_form) : H HA :=
+  eval_rec val (proof s) (Vnil (H HA)).
+
+Fixpoint valid_ctx_from_list (A : list valid_form) : is_valid_ctx 0 (map f A) :=
   match A with
-  |[] => s
-  |a::A => (revert A (a ~> s))
+  | [] => Valid_nil 0
+  | s::A => Valid_cons (proof s) (valid_ctx_from_list A)
   end.
 
-Lemma revert_correct A s :
-  A |- s <-> [] |- revert A s.
+Fixpoint Meet_list {HA} (val : nat -> H HA) (A : list valid_form) : H HA :=
+  match A with
+  | [] => impl (bottom HA) (bottom HA)
+  | s::A => meet (eval val s) (Meet_list val A)
+  end.
+
+Lemma Meet_list_equivalence {HA} (val : nat -> H HA) (A : list valid_form) :
+  Meet_list val A = Meet_valid_ctx val (valid_ctx_from_list A) (Vnil (H HA)).
 Proof.
-  split; revert s. 
-  - induction A; intros s H.
-    + unfold revert. assumption.
-    + simpl. apply IHA.
-      apply Iimp. assumption.
-  - induction A; intros s H.
-    + unfold revert in H. assumption.
-    + apply Eimp with (s := a). 
-      * apply Ass. apply in_eq.
-      * apply Weak with (A := A).
-        apply IHA. apply H.
-        apply incl_tl. apply incl_refl.
-Qed.
-
-(** 2.g *)
-Definition HA_leq := fun s t => [] |- s ~> t.
-Definition HA_bot := bot.
-Definition HA_impl s t := imp s t. 
-Definition HA_meet s t := conj s t.
-
-Lemma HA_leq_refl (s : form) :
-  HA_leq s s.
-Proof.
-  unfold HA_leq.
-  apply Iimp.
-  apply Ass.
-  apply in_eq.
-Qed.
-
-Lemma HA_leq_trans (s t u : form) :
-  HA_leq s t -> HA_leq t u -> HA_leq s u.
-Proof.
-  unfold HA_leq.
-  intros H1 H2.
-  apply Iimp.
-  apply Eimp with (s := t).
-  - apply Eimp with (s := s).
-    + apply Ass. apply in_eq.
-    + apply Weak with (A := []). 
-      * assumption. 
-      * apply incl_tl. apply incl_refl.
-  - apply Weak with (A := []).
-    + assumption.
-    + apply incl_tl. apply incl_refl.
-Qed.
-
-Lemma HA_leq_bottom (u : form) :
-  HA_leq HA_bot u.
-Proof.
-  unfold HA_leq. unfold HA_bot.
-  apply Iimp.
-  apply Exp.
-  apply Ass. apply in_eq.
-Qed.
-
-Lemma HA_leq_meet (s t u : form) :
-  HA_leq u s /\ HA_leq u t <-> HA_leq u (HA_meet s t).
-Proof.
-  unfold HA_leq. unfold HA_meet.
-  split; intro H.
-  - destruct H. 
-    apply Iimp. apply Iconj.
-    + apply Eimp with (s := u).
-      * apply Ass. apply in_eq.
-      * apply Weak with (A := []).
-        assumption.
-        apply incl_tl. apply incl_refl.
-    + apply Eimp with (s := u).
-      * apply Ass. apply in_eq.
-      * apply Weak with (A := []).
-        assumption.
-        apply incl_tl. apply incl_refl.
-  - split.
-    + apply Iimp. 
-      apply Econjl with (t := t).
-      apply Eimp with (s := u).
-      * apply Ass. apply in_eq.
-      * apply Weak with (A := []).
-        assumption.
-        apply incl_tl. apply incl_refl.
-    + apply Iimp. 
-      apply Econjr with (s := s).
-      apply Eimp with (s := u).
-      * apply Ass. apply in_eq.
-      * apply Weak with (A := []).
-        assumption.
-        apply incl_tl. apply incl_refl.
-Qed.
-
-Lemma HA_leq_impl (s t u : form) :
-  (HA_leq (HA_meet s t) u) <-> HA_leq s (HA_impl t u).
-Proof.
-  unfold HA_leq. unfold HA_meet. unfold HA_impl.
-  split; intro H.
-  - apply Iimp. apply Iimp. 
-    apply Eimp with (s := conj s t).
-    + apply Iconj.
-      * apply Ass. apply in_cons. apply in_eq.
-      * apply Ass. apply in_eq.
-    + apply Weak with (A := []).
-      * assumption.
-      * apply incl_tl. apply incl_tl. apply incl_refl.
-  - apply Iimp.
-    apply Eimp with (s := t).
-    + apply Econjr with (s := s).
-      apply Ass. apply in_eq.
-    + apply Eimp with (s := s).
-      * apply Econjl with (t := t).
-        apply Ass. apply in_eq.
-      * apply Weak with (A := []).
-        assumption.
-        apply incl_tl. apply incl_refl.
-Qed.
-
-Definition HA_formula : HeytingAlgebra :=
-{| H := form;
-  leq := HA_leq;
-  leq_refl := HA_leq_refl;
-  leq_trans := HA_leq_trans;
-  bottom := HA_bot;
-  meet := HA_meet;
-  impl := HA_impl;
-  leq_bottom := HA_leq_bottom;
-  leq_meet := HA_leq_meet;
-  leq_impl := HA_leq_impl
-|}.
-
-(** 2.h *)
-Lemma eval_is_id (s : form) :
-  eval (HA:=HA_formula) var s = s.
-Proof.
-  induction s.
+  induction A.
   - reflexivity.
-  - reflexivity.
-  - simpl eval. rewrite IHs1. rewrite IHs2. reflexivity.
-  - simpl eval. rewrite IHs1. rewrite IHs2. reflexivity.
-Qed.
-
-(** 2.i *)
-(*Lemma Heyting_completeness *)
-
-Lemma revert_HA (HA : HeytingAlgebra) (val : nat -> H HA) A s :
-  hent val A s <-> hent val [] (revert A s).
-Proof.
-  split; revert s; induction A; intros s H.
-  - assumption.
   - simpl.
-    apply IHA.
-    apply leq_impl.
-    apply leq_trans with (t := meet (eval val a) (Meet_list val A)).
-    + apply leq_meet; split; 
-      apply (leq_meet (Meet_list val A) (eval val a) (meet (Meet_list val A) (eval val a)));
-      apply leq_refl.
-    + assumption.
-  - assumption.
-  - apply leq_trans with (t := meet (Meet_list val A) (eval val a)).
-    + apply leq_meet; split;
-      apply (leq_meet (eval val a) (Meet_list val A) (meet (eval val a) (Meet_list val A)));
-      apply leq_refl.
-    + apply leq_impl.
-      apply IHA with (s := a ~> s).
-      assumption.
+    apply f_equal2.
+    + rewrite eval_rec_proof_irrelevance with (p := proj1 (valid_cons_eq (Valid_cons (proof a) (valid_ctx_from_list A)))) (q := proof a).
+      reflexivity.
+    + rewrite Meet_valid_ctx_proof_irrelevance with (p := proj2 (valid_cons_eq (Valid_cons (proof a) (valid_ctx_from_list A)))) (q := valid_ctx_from_list A).
+      apply IHA.
 Qed.
 
-Proposition nd_completeHA A s :
-  (forall (HA : HeytingAlgebra) (V : nat -> H HA), hent V A s) -> nd A s.
+Definition hent {HA} (val : nat -> H HA) (A : list valid_form) (s : valid_form) := leq (Meet_list val A) (eval val s).
+
+Lemma nd_soundHA {HA} (val : nat -> H HA) (A : list valid_form) (s : valid_form) :
+  nd (map f A) (f s) -> hent val A s.
 Proof.
-  intro H.
-  apply revert_correct.
-  apply Eimp with (s := bot ~> bot).
-  - apply Iimp. apply Ass. apply in_eq.
-  - specialize H with (HA := HA_formula) (V := var).
-    apply revert_HA in H.
-    simpl in H.
-    rewrite eval_is_id in H.
-    assumption.
+  intro ND.
+  unfold hent.
+  rewrite Meet_list_equivalence.
+  unfold eval.
+  apply nd_soundHA_rec.
+  apply ND.
 Qed.
-
-Theorem HA_iff_nd A s:
-(forall (HA : HeytingAlgebra) (V : nat -> H HA), hent V A s) <-> nd A s.
-Proof.
-  split.
-  - apply nd_completeHA.
-  - intros H HA V.
-    apply nd_soundHA.
-    assumption.
-Qed.
-
-
-
-
-
-
 
 
 
